stage0/stdlib/Init/Data/ToString/Macro.c
@@ -37,6 +37,7 @@ extern lean_object* l_Lean_instInhabitedSourceInfo___closed__1;
 lean_object* l___kind_term____x40_Init_Data_ToString_Macro___hyg_2____closed__1;
 lean_object* l___kind_term____x40_Init_Data_ToString_Macro___hyg_2____closed__2;
 extern lean_object* l___kind_term____x40_Init_Notation___hyg_5672____closed__9;
+extern lean_object* l___kind_term____x40_Init_Data_Array_Basic___hyg_3338____closed__2;
 lean_object* l___kind_term____x40_Init_Data_ToString_Macro___hyg_2____closed__9;
 lean_object* l___kind_term____x40_Init_Data_ToString_Macro___hyg_2____closed__13;
 lean_object* l_myMacro____x40_Init_Data_ToString_Macro___hyg_43____closed__9;
@@ -50,7 +51,6 @@ lean_object* l_myMacro____x40_Init_Data_ToString_Macro___hyg_43____closed__1;
 extern lean_object* l_Lean_Name_hasMacroScopes___closed__1;
 lean_object* l___kind_term____x40_Init_Data_ToString_Macro___hyg_2____closed__3;
 lean_object* lean_name_mk_numeral(lean_object*, lean_object*);
-extern lean_object* l___kind_term____x40_Init_Data_Array_Basic___hyg_3349____closed__2;
 uint8_t l_Lean_Syntax_isOfKind(lean_object*, lean_object*);
 lean_object* l___kind_term____x40_Init_Data_ToString_Macro___hyg_2____closed__7;
 lean_object* l_Lean_Syntax_getArg(lean_object*, lean_object*);
@@ -69,7 +69,7 @@ static lean_object* _init_l___kind_term____x40_Init_Data_ToString_Macro___hyg_2_
 _start:
 {
 lean_object* x_1; lean_object* x_2; lean_object* x_3; 
-x_1 = l___kind_term____x40_Init_Data_Array_Basic___hyg_3349____closed__2;
+x_1 = l___kind_term____x40_Init_Data_Array_Basic___hyg_3338____closed__2;
 x_2 = l___kind_term____x40_Init_Data_ToString_Macro___hyg_2____closed__1;
 x_3 = lean_name_mk_string(x_1, x_2);
 return x_3;
