stage0/stdlib/Lean/Elab/App.c
@@ -580,7 +580,7 @@ lean_object* l_Lean_Elab_getRefPos___at___private_Lean_Elab_App_0__Lean_Elab_Ter
 lean_object* l___regBuiltin_Lean_Elab_Term_elabChoice___closed__1;
 lean_object* l___private_Lean_Elab_App_0__Lean_Elab_Term_ElabAppArgs_finalize___lambda__1(lean_object*, lean_object*, lean_object*, lean_object*, lean_object*, lean_object*, lean_object*, lean_object*, lean_object*, lean_object*);
 lean_object* l___private_Lean_Elab_App_0__Lean_Elab_Term_ElabAppArgs_getForallBody___lambda__1___boxed(lean_object*, lean_object*);
-lean_object* l_Lean_Elab_Term_initFn____x40_Lean_Elab_App___hyg_7555_(lean_object*);
+lean_object* l_Lean_Elab_Term_initFn____x40_Lean_Elab_App___hyg_7569_(lean_object*);
 lean_object* l___private_Lean_Elab_App_0__Lean_Elab_Term_elabAppAux(lean_object*, lean_object*, lean_object*, uint8_t, lean_object*, lean_object*, lean_object*, lean_object*, lean_object*, lean_object*, lean_object*, lean_object*);
 extern lean_object* l_myMacro____x40_Init_Notation___hyg_8168____closed__12;
 lean_object* l_Lean_mkForall(lean_object*, uint8_t, lean_object*, lean_object*);
@@ -13315,23 +13315,29 @@ return x_2;
 lean_object* l___private_Lean_Elab_App_0__Lean_Elab_Term_ElabAppArgs_propagateExpectedType(lean_object* x_1, lean_object* x_2, lean_object* x_3, lean_object* x_4, lean_object* x_5, lean_object* x_6, lean_object* x_7, lean_object* x_8) {
 _start:
 {
-lean_object* x_9; uint8_t x_10; 
+lean_object* x_9; lean_object* x_10; lean_object* x_11; lean_object* x_12; uint8_t x_13; lean_object* x_14; uint8_t x_15; 
 x_9 = lean_st_ref_get(x_1, x_8);
-x_10 = !lean_is_exclusive(x_9);
-if (x_10 == 0)
-{
-lean_object* x_11; lean_object* x_12; uint8_t x_13; lean_object* x_14; uint8_t x_15; 
-x_11 = lean_ctor_get(x_9, 0);
-x_12 = lean_ctor_get(x_9, 1);
-x_13 = lean_ctor_get_uint8(x_11, sizeof(void*)*9);
-x_14 = lean_ctor_get(x_11, 5);
+x_10 = lean_ctor_get(x_9, 0);
+lean_inc(x_10);
+x_11 = lean_ctor_get(x_9, 1);
+lean_inc(x_11);
+if (lean_is_exclusive(x_9)) {
+ lean_ctor_release(x_9, 0);
+ lean_ctor_release(x_9, 1);
+ x_12 = x_9;
+} else {
+ lean_dec_ref(x_9);
+ x_12 = lean_box(0);
+}
+x_13 = lean_ctor_get_uint8(x_10, sizeof(void*)*9);
+x_14 = lean_ctor_get(x_10, 5);
 lean_inc(x_14);
 x_15 = l_Array_isEmpty___rarg(x_14);
 if (x_15 == 0)
 {
-lean_object* x_16; 
+lean_object* x_16; lean_object* x_17; 
 lean_dec(x_14);
-lean_dec(x_11);
+lean_dec(x_10);
 lean_dec(x_7);
 lean_dec(x_6);
 lean_dec(x_5);
@@ -13340,46 +13346,38 @@ lean_dec(x_3);
 lean_dec(x_2);
 lean_dec(x_1);
 x_16 = lean_box(0);
-lean_ctor_set(x_9, 0, x_16);
-return x_9;
+if (lean_is_scalar(x_12)) {
+ x_17 = lean_alloc_ctor(0, 2, 0);
+} else {
+ x_17 = x_12;
+}
+lean_ctor_set(x_17, 0, x_16);
+lean_ctor_set(x_17, 1, x_11);
+return x_17;
 }
 else
 {
 if (x_13 == 0)
 {
-uint8_t x_17; 
-x_17 = lean_ctor_get_uint8(x_11, sizeof(void*)*9 + 2);
-if (x_17 == 0)
+uint8_t x_18; 
+x_18 = lean_ctor_get_uint8(x_10, sizeof(void*)*9 + 2);
+if (x_18 == 0)
 {
-lean_object* x_18; uint8_t x_19; 
-x_18 = lean_ctor_get(x_11, 8);
-lean_inc(x_18);
-x_19 = l_Array_isEmpty___rarg(x_18);
-if (x_19 == 0)
+lean_object* x_19; uint8_t x_20; 
+x_19 = lean_ctor_get(x_10, 8);
+lean_inc(x_19);
+x_20 = l_Array_isEmpty___rarg(x_19);
+if (x_20 == 0)
 {
-lean_object* x_20; lean_object* x_21; lean_object* x_22; uint8_t x_23; 
-lean_free_object(x_9);
-x_20 = lean_st_ref_take(x_1, x_12);
-x_21 = lean_ctor_get(x_20, 0);
+lean_object* x_21; 
+x_21 = lean_ctor_get(x_10, 4);
 lean_inc(x_21);
-x_22 = lean_ctor_get(x_20, 1);
-lean_inc(x_22);
-lean_dec(x_20);
-x_23 = !lean_is_exclusive(x_21);
-if (x_23 == 0)
+if (lean_obj_tag(x_21) == 0)
 {
-uint8_t x_24; lean_object* x_25; lean_object* x_26; 
-x_24 = 1;
-lean_ctor_set_uint8(x_21, sizeof(void*)*9 + 2, x_24);
-x_25 = lean_st_ref_set(x_1, x_21, x_22);
-x_26 = lean_ctor_get(x_11, 4);
-lean_inc(x_26);
-if (lean_obj_tag(x_26) == 0)
-{
-uint8_t x_27; 
-lean_dec(x_18);
+lean_object* x_22; lean_object* x_23; 
+lean_dec(x_19);
 lean_dec(x_14);
-lean_dec(x_11);
+lean_dec(x_10);
 lean_dec(x_7);
 lean_dec(x_6);
 lean_dec(x_5);
@@ -13387,106 +13385,215 @@ lean_dec(x_4);
 lean_dec(x_3);
 lean_dec(x_2);
 lean_dec(x_1);
-x_27 = !lean_is_exclusive(x_25);
-if (x_27 == 0)
-{
-lean_object* x_28; lean_object* x_29; 
-x_28 = lean_ctor_get(x_25, 0);
-lean_dec(x_28);
-x_29 = lean_box(0);
-lean_ctor_set(x_25, 0, x_29);
-return x_25;
+x_22 = lean_box(0);
+if (lean_is_scalar(x_12)) {
+ x_23 = lean_alloc_ctor(0, 2, 0);
+} else {
+ x_23 = x_12;
+}
+lean_ctor_set(x_23, 0, x_22);
+lean_ctor_set(x_23, 1, x_11);
+return x_23;
 }
 else
+{
+lean_object* x_24; uint8_t x_25; 
+x_24 = lean_ctor_get(x_21, 0);
+lean_inc(x_24);
+lean_dec(x_21);
+x_25 = l_Lean_Expr_isProp(x_24);
+if (x_25 == 0)
+{
+lean_object* x_26; lean_object* x_27; lean_object* x_28; lean_object* x_29; uint8_t x_197; lean_object* x_198; lean_object* x_220; lean_object* x_221; lean_object* x_222; uint8_t x_223; 
+x_26 = lean_ctor_get(x_10, 2);
+lean_inc(x_26);
+x_27 = lean_unsigned_to_nat(0u);
+x_28 = l_List_lengthAux___rarg(x_26, x_27);
+lean_dec(x_26);
+x_220 = lean_st_ref_get(x_7, x_11);
+x_221 = lean_ctor_get(x_220, 0);
+lean_inc(x_221);
+x_222 = lean_ctor_get(x_221, 3);
+lean_inc(x_222);
+lean_dec(x_221);
+x_223 = lean_ctor_get_uint8(x_222, sizeof(void*)*1);
+lean_dec(x_222);
+if (x_223 == 0)
+{
+lean_object* x_224; uint8_t x_225; 
+x_224 = lean_ctor_get(x_220, 1);
+lean_inc(x_224);
+lean_dec(x_220);
+x_225 = 0;
+x_197 = x_225;
+x_198 = x_224;
+goto block_219;
+}
+else
+{
+lean_object* x_226; lean_object* x_227; lean_object* x_228; lean_object* x_229; lean_object* x_230; uint8_t x_231; 
+x_226 = lean_ctor_get(x_220, 1);
+lean_inc(x_226);
+lean_dec(x_220);
+x_227 = l___private_Lean_Elab_App_0__Lean_Elab_Term_ElabAppArgs_propagateExpectedType___closed__3;
+x_228 = l___private_Lean_Util_Trace_0__Lean_checkTraceOptionM___at___private_Lean_Elab_App_0__Lean_Elab_Term_ElabAppArgs_propagateExpectedType___spec__7(x_227, x_1, x_2, x_3, x_4, x_5, x_6, x_7, x_226);
+x_229 = lean_ctor_get(x_228, 0);
+lean_inc(x_229);
+x_230 = lean_ctor_get(x_228, 1);
+lean_inc(x_230);
+lean_dec(x_228);
+x_231 = lean_unbox(x_229);
+lean_dec(x_229);
+x_197 = x_231;
+x_198 = x_230;
+goto block_219;
+}
+block_196:
 {
 lean_object* x_30; lean_object* x_31; lean_object* x_32; 
-x_30 = lean_ctor_get(x_25, 1);
+x_30 = lean_ctor_get(x_10, 3);
 lean_inc(x_30);
-lean_dec(x_25);
-x_31 = lean_box(0);
-x_32 = lean_alloc_ctor(0, 2, 0);
-lean_ctor_set(x_32, 0, x_31);
-lean_ctor_set(x_32, 1, x_30);
-return x_32;
+x_31 = lean_ctor_get(x_10, 1);
+lean_inc(x_31);
+x_32 = l___private_Lean_Elab_App_0__Lean_Elab_Term_ElabAppArgs_getForallBody(x_28, x_30, x_31);
+if (lean_obj_tag(x_32) == 0)
+{
+lean_object* x_33; lean_object* x_34; 
+lean_dec(x_24);
+lean_dec(x_19);
+lean_dec(x_10);
+lean_dec(x_7);
+lean_dec(x_6);
+lean_dec(x_5);
+lean_dec(x_4);
+lean_dec(x_3);
+lean_dec(x_2);
+lean_dec(x_1);
+x_33 = lean_box(0);
+if (lean_is_scalar(x_12)) {
+ x_34 = lean_alloc_ctor(0, 2, 0);
+} else {
+ x_34 = x_12;
 }
+lean_ctor_set(x_34, 0, x_33);
+lean_ctor_set(x_34, 1, x_29);
+return x_34;
 }
 else
 {
-lean_object* x_33; lean_object* x_34; lean_object* x_35; uint8_t x_36; 
-x_33 = lean_ctor_get(x_25, 1);
-lean_inc(x_33);
-if (lean_is_exclusive(x_25)) {
- lean_ctor_release(x_25, 0);
- lean_ctor_release(x_25, 1);
- x_34 = x_25;
-} else {
- lean_dec_ref(x_25);
- x_34 = lean_box(0);
-}
-x_35 = lean_ctor_get(x_26, 0);
+lean_object* x_35; uint8_t x_36; 
+x_35 = lean_ctor_get(x_32, 0);
 lean_inc(x_35);
-lean_dec(x_26);
-x_36 = l_Lean_Expr_isProp(x_35);
+lean_dec(x_32);
+x_36 = l_Lean_Expr_hasLooseBVars(x_35);
 if (x_36 == 0)
 {
-lean_object* x_37; lean_object* x_38; lean_object* x_39; lean_object* x_40; uint8_t x_166; lean_object* x_167; lean_object* x_189; lean_object* x_190; lean_object* x_191; uint8_t x_192; 
-x_37 = lean_ctor_get(x_11, 2);
-lean_inc(x_37);
-x_38 = lean_unsigned_to_nat(0u);
-x_39 = l_List_lengthAux___rarg(x_37, x_38);
-lean_dec(x_37);
-x_189 = lean_st_ref_get(x_7, x_33);
-x_190 = lean_ctor_get(x_189, 0);
-lean_inc(x_190);
-x_191 = lean_ctor_get(x_190, 3);
-lean_inc(x_191);
-lean_dec(x_190);
-x_192 = lean_ctor_get_uint8(x_191, sizeof(void*)*1);
-lean_dec(x_191);
-if (x_192 == 0)
+lean_object* x_37; lean_object* x_38; 
+x_37 = lean_box(0);
+lean_inc(x_35);
+x_38 = l_Lean_FindMVar_main___at___private_Lean_Elab_App_0__Lean_Elab_Term_ElabAppArgs_propagateExpectedType___spec__1(x_10, x_35, x_37);
+if (lean_obj_tag(x_38) == 0)
 {
-lean_object* x_193; uint8_t x_194; 
-x_193 = lean_ctor_get(x_189, 1);
-lean_inc(x_193);
-lean_dec(x_189);
-x_194 = 0;
-x_166 = x_194;
-x_167 = x_193;
-goto block_188;
+lean_object* x_39; lean_object* x_40; 
+lean_dec(x_35);
+lean_dec(x_24);
+lean_dec(x_19);
+lean_dec(x_7);
+lean_dec(x_6);
+lean_dec(x_5);
+lean_dec(x_4);
+lean_dec(x_3);
+lean_dec(x_2);
+lean_dec(x_1);
+x_39 = lean_box(0);
+if (lean_is_scalar(x_12)) {
+ x_40 = lean_alloc_ctor(0, 2, 0);
+} else {
+ x_40 = x_12;
+}
+lean_ctor_set(x_40, 0, x_39);
+lean_ctor_set(x_40, 1, x_29);
+return x_40;
 }
 else
 {
-lean_object* x_195; lean_object* x_196; lean_object* x_197; lean_object* x_198; lean_object* x_199; uint8_t x_200; 
-x_195 = lean_ctor_get(x_189, 1);
-lean_inc(x_195);
-lean_dec(x_189);
-x_196 = l___private_Lean_Elab_App_0__Lean_Elab_Term_ElabAppArgs_propagateExpectedType___closed__3;
-x_197 = l___private_Lean_Util_Trace_0__Lean_checkTraceOptionM___at___private_Lean_Elab_App_0__Lean_Elab_Term_ElabAppArgs_propagateExpectedType___spec__7(x_196, x_1, x_2, x_3, x_4, x_5, x_6, x_7, x_195);
-x_198 = lean_ctor_get(x_197, 0);
-lean_inc(x_198);
-x_199 = lean_ctor_get(x_197, 1);
-lean_inc(x_199);
-lean_dec(x_197);
-x_200 = lean_unbox(x_198);
-lean_dec(x_198);
-x_166 = x_200;
-x_167 = x_199;
-goto block_188;
-}
-block_165:
+lean_object* x_41; 
+lean_dec(x_38);
+lean_inc(x_35);
+x_41 = l_Lean_FindMVar_main___at___private_Lean_Elab_App_0__Lean_Elab_Term_ElabAppArgs_propagateExpectedType___spec__2(x_19, x_35, x_37);
+if (lean_obj_tag(x_41) == 0)
 {
-lean_object* x_41; lean_object* x_42; lean_object* x_43; 
-x_41 = lean_ctor_get(x_11, 3);
-lean_inc(x_41);
-x_42 = lean_ctor_get(x_11, 1);
-lean_inc(x_42);
-x_43 = l___private_Lean_Elab_App_0__Lean_Elab_Term_ElabAppArgs_getForallBody(x_39, x_41, x_42);
+lean_object* x_42; lean_object* x_43; 
+lean_dec(x_12);
+x_42 = l___private_Lean_Elab_App_0__Lean_Elab_Term_ElabAppArgs_hasOptAutoParams___closed__1;
+lean_inc(x_7);
+lean_inc(x_6);
+lean_inc(x_5);
+lean_inc(x_4);
+lean_inc(x_3);
+lean_inc(x_2);
+lean_inc(x_1);
+lean_inc(x_35);
+x_43 = l_Lean_Meta_forallTelescopeReducing___at___private_Lean_Elab_App_0__Lean_Elab_Term_ElabAppArgs_hasOptAutoParams___spec__2___rarg(x_35, x_42, x_1, x_2, x_3, x_4, x_5, x_6, x_7, x_29);
 if (lean_obj_tag(x_43) == 0)
 {
-lean_object* x_44; lean_object* x_45; 
+uint8_t x_44; 
+x_44 = !lean_is_exclusive(x_43);
+if (x_44 == 0)
+{
+lean_object* x_45; lean_object* x_46; lean_object* x_47; uint8_t x_93; lean_object* x_94; uint8_t x_107; 
+x_45 = lean_ctor_get(x_43, 0);
+x_46 = lean_ctor_get(x_43, 1);
+x_107 = lean_unbox(x_45);
+lean_dec(x_45);
+if (x_107 == 0)
+{
+lean_object* x_108; lean_object* x_109; lean_object* x_110; uint8_t x_111; 
+lean_free_object(x_43);
+x_108 = lean_st_ref_get(x_7, x_46);
+x_109 = lean_ctor_get(x_108, 0);
+lean_inc(x_109);
+x_110 = lean_ctor_get(x_109, 3);
+lean_inc(x_110);
+lean_dec(x_109);
+x_111 = lean_ctor_get_uint8(x_110, sizeof(void*)*1);
+lean_dec(x_110);
+if (x_111 == 0)
+{
+lean_object* x_112; uint8_t x_113; 
+x_112 = lean_ctor_get(x_108, 1);
+lean_inc(x_112);
+lean_dec(x_108);
+x_113 = 0;
+x_93 = x_113;
+x_94 = x_112;
+goto block_106;
+}
+else
+{
+lean_object* x_114; lean_object* x_115; lean_object* x_116; lean_object* x_117; lean_object* x_118; uint8_t x_119; 
+x_114 = lean_ctor_get(x_108, 1);
+lean_inc(x_114);
+lean_dec(x_108);
+x_115 = l___private_Lean_Elab_App_0__Lean_Elab_Term_ElabAppArgs_propagateExpectedType___closed__3;
+x_116 = l___private_Lean_Util_Trace_0__Lean_checkTraceOptionM___at___private_Lean_Elab_App_0__Lean_Elab_Term_ElabAppArgs_propagateExpectedType___spec__7(x_115, x_1, x_2, x_3, x_4, x_5, x_6, x_7, x_114);
+x_117 = lean_ctor_get(x_116, 0);
+lean_inc(x_117);
+x_118 = lean_ctor_get(x_116, 1);
+lean_inc(x_118);
+lean_dec(x_116);
+x_119 = lean_unbox(x_117);
+lean_dec(x_117);
+x_93 = x_119;
+x_94 = x_118;
+goto block_106;
+}
+}
+else
+{
+lean_object* x_120; 
 lean_dec(x_35);
-lean_dec(x_18);
-lean_dec(x_11);
+lean_dec(x_24);
 lean_dec(x_7);
 lean_dec(x_6);
 lean_dec(x_5);
@@ -13494,639 +13601,276 @@ lean_dec(x_4);
 lean_dec(x_3);
 lean_dec(x_2);
 lean_dec(x_1);
-x_44 = lean_box(0);
-if (lean_is_scalar(x_34)) {
- x_45 = lean_alloc_ctor(0, 2, 0);
-} else {
- x_45 = x_34;
+x_120 = lean_box(0);
+lean_ctor_set(x_43, 0, x_120);
+return x_43;
 }
-lean_ctor_set(x_45, 0, x_44);
-lean_ctor_set(x_45, 1, x_40);
-return x_45;
-}
-else
+block_92:
 {
-lean_object* x_46; uint8_t x_47; 
-x_46 = lean_ctor_get(x_43, 0);
-lean_inc(x_46);
-lean_dec(x_43);
-x_47 = l_Lean_Expr_hasLooseBVars(x_46);
-if (x_47 == 0)
-{
-lean_object* x_48; lean_object* x_49; 
-x_48 = lean_box(0);
-lean_inc(x_46);
-x_49 = l_Lean_FindMVar_main___at___private_Lean_Elab_App_0__Lean_Elab_Term_ElabAppArgs_propagateExpectedType___spec__1(x_11, x_46, x_48);
-if (lean_obj_tag(x_49) == 0)
-{
-lean_object* x_50; lean_object* x_51; 
-lean_dec(x_46);
-lean_dec(x_35);
-lean_dec(x_18);
-lean_dec(x_7);
-lean_dec(x_6);
-lean_dec(x_5);
-lean_dec(x_4);
+lean_object* x_48; 
+x_48 = l_Lean_Meta_isExprDefEq___at___private_Lean_Elab_App_0__Lean_Elab_Term_ElabAppArgs_propagateExpectedType___spec__3(x_24, x_35, x_1, x_2, x_3, x_4, x_5, x_6, x_7, x_47);
 lean_dec(x_3);
 lean_dec(x_2);
-lean_dec(x_1);
-x_50 = lean_box(0);
-if (lean_is_scalar(x_34)) {
- x_51 = lean_alloc_ctor(0, 2, 0);
-} else {
- x_51 = x_34;
-}
-lean_ctor_set(x_51, 0, x_50);
-lean_ctor_set(x_51, 1, x_40);
-return x_51;
-}
-else
+if (lean_obj_tag(x_48) == 0)
 {
-lean_object* x_52; 
+lean_object* x_49; uint8_t x_50; 
+x_49 = lean_ctor_get(x_48, 0);
+lean_inc(x_49);
+x_50 = lean_unbox(x_49);
 lean_dec(x_49);
-lean_inc(x_46);
-x_52 = l_Lean_FindMVar_main___at___private_Lean_Elab_App_0__Lean_Elab_Term_ElabAppArgs_propagateExpectedType___spec__2(x_18, x_46, x_48);
-if (lean_obj_tag(x_52) == 0)
+if (x_50 == 0)
 {
-lean_object* x_53; lean_object* x_54; 
-lean_dec(x_34);
-x_53 = l___private_Lean_Elab_App_0__Lean_Elab_Term_ElabAppArgs_hasOptAutoParams___closed__1;
-lean_inc(x_7);
-lean_inc(x_6);
-lean_inc(x_5);
-lean_inc(x_4);
-lean_inc(x_3);
-lean_inc(x_2);
-lean_inc(x_1);
-lean_inc(x_46);
-x_54 = l_Lean_Meta_forallTelescopeReducing___at___private_Lean_Elab_App_0__Lean_Elab_Term_ElabAppArgs_hasOptAutoParams___spec__2___rarg(x_46, x_53, x_1, x_2, x_3, x_4, x_5, x_6, x_7, x_40);
-if (lean_obj_tag(x_54) == 0)
+uint8_t x_51; 
+lean_dec(x_1);
+x_51 = !lean_is_exclusive(x_48);
+if (x_51 == 0)
 {
-uint8_t x_55; 
-x_55 = !lean_is_exclusive(x_54);
-if (x_55 == 0)
-{
-lean_object* x_56; lean_object* x_57; uint8_t x_58; lean_object* x_59; uint8_t x_94; 
-x_56 = lean_ctor_get(x_54, 0);
-x_57 = lean_ctor_get(x_54, 1);
-x_94 = lean_unbox(x_56);
-lean_dec(x_56);
-if (x_94 == 0)
-{
-lean_object* x_95; lean_object* x_96; lean_object* x_97; uint8_t x_98; 
-lean_free_object(x_54);
-x_95 = lean_st_ref_get(x_7, x_57);
-x_96 = lean_ctor_get(x_95, 0);
-lean_inc(x_96);
-x_97 = lean_ctor_get(x_96, 3);
-lean_inc(x_97);
-lean_dec(x_96);
-x_98 = lean_ctor_get_uint8(x_97, sizeof(void*)*1);
-lean_dec(x_97);
-if (x_98 == 0)
-{
-lean_object* x_99; uint8_t x_100; 
-x_99 = lean_ctor_get(x_95, 1);
-lean_inc(x_99);
-lean_dec(x_95);
-x_100 = 0;
-x_58 = x_100;
-x_59 = x_99;
-goto block_93;
+lean_object* x_52; lean_object* x_53; 
+x_52 = lean_ctor_get(x_48, 0);
+lean_dec(x_52);
+x_53 = lean_box(0);
+lean_ctor_set(x_48, 0, x_53);
+return x_48;
 }
 else
 {
-lean_object* x_101; lean_object* x_102; lean_object* x_103; lean_object* x_104; lean_object* x_105; uint8_t x_106; 
-x_101 = lean_ctor_get(x_95, 1);
-lean_inc(x_101);
-lean_dec(x_95);
-x_102 = l___private_Lean_Elab_App_0__Lean_Elab_Term_ElabAppArgs_propagateExpectedType___closed__3;
-x_103 = l___private_Lean_Util_Trace_0__Lean_checkTraceOptionM___at___private_Lean_Elab_App_0__Lean_Elab_Term_ElabAppArgs_propagateExpectedType___spec__7(x_102, x_1, x_2, x_3, x_4, x_5, x_6, x_7, x_101);
-x_104 = lean_ctor_get(x_103, 0);
-lean_inc(x_104);
-x_105 = lean_ctor_get(x_103, 1);
-lean_inc(x_105);
-lean_dec(x_103);
-x_106 = lean_unbox(x_104);
-lean_dec(x_104);
-x_58 = x_106;
-x_59 = x_105;
-goto block_93;
+lean_object* x_54; lean_object* x_55; lean_object* x_56; 
+x_54 = lean_ctor_get(x_48, 1);
+lean_inc(x_54);
+lean_dec(x_48);
+x_55 = lean_box(0);
+x_56 = lean_alloc_ctor(0, 2, 0);
+lean_ctor_set(x_56, 0, x_55);
+lean_ctor_set(x_56, 1, x_54);
+return x_56;
 }
 }
 else
 {
-lean_object* x_107; 
-lean_dec(x_46);
-lean_dec(x_35);
-lean_dec(x_7);
-lean_dec(x_6);
-lean_dec(x_5);
-lean_dec(x_4);
-lean_dec(x_3);
-lean_dec(x_2);
-lean_dec(x_1);
-x_107 = lean_box(0);
-lean_ctor_set(x_54, 0, x_107);
-return x_54;
-}
-block_93:
-{
-if (x_58 == 0)
-{
-lean_object* x_60; 
-x_60 = l_Lean_Meta_isExprDefEq___at___private_Lean_Elab_App_0__Lean_Elab_Term_ElabAppArgs_propagateExpectedType___spec__3(x_35, x_46, x_1, x_2, x_3, x_4, x_5, x_6, x_7, x_59);
-lean_dec(x_3);
-lean_dec(x_2);
-lean_dec(x_1);
-if (lean_obj_tag(x_60) == 0)
-{
-uint8_t x_61; 
-x_61 = !lean_is_exclusive(x_60);
+lean_object* x_57; lean_object* x_58; lean_object* x_59; lean_object* x_60; uint8_t x_61; 
+x_57 = lean_ctor_get(x_48, 1);
+lean_inc(x_57);
+lean_dec(x_48);
+x_58 = lean_st_ref_take(x_1, x_57);
+x_59 = lean_ctor_get(x_58, 0);
+lean_inc(x_59);
+x_60 = lean_ctor_get(x_58, 1);
+lean_inc(x_60);
+lean_dec(x_58);
+x_61 = !lean_is_exclusive(x_59);
 if (x_61 == 0)
 {
-lean_object* x_62; lean_object* x_63; 
-x_62 = lean_ctor_get(x_60, 0);
-lean_dec(x_62);
-x_63 = lean_box(0);
-lean_ctor_set(x_60, 0, x_63);
-return x_60;
-}
-else
-{
-lean_object* x_64; lean_object* x_65; lean_object* x_66; 
-x_64 = lean_ctor_get(x_60, 1);
-lean_inc(x_64);
-lean_dec(x_60);
-x_65 = lean_box(0);
-x_66 = lean_alloc_ctor(0, 2, 0);
-lean_ctor_set(x_66, 0, x_65);
-lean_ctor_set(x_66, 1, x_64);
-return x_66;
-}
-}
-else
-{
-uint8_t x_67; 
-x_67 = !lean_is_exclusive(x_60);
-if (x_67 == 0)
-{
-return x_60;
-}
-else
-{
-lean_object* x_68; lean_object* x_69; lean_object* x_70; 
-x_68 = lean_ctor_get(x_60, 0);
-x_69 = lean_ctor_get(x_60, 1);
-lean_inc(x_69);
-lean_inc(x_68);
-lean_dec(x_60);
-x_70 = lean_alloc_ctor(1, 2, 0);
-lean_ctor_set(x_70, 0, x_68);
-lean_ctor_set(x_70, 1, x_69);
-return x_70;
-}
-}
-}
-else
-{
-lean_object* x_71; lean_object* x_72; lean_object* x_73; lean_object* x_74; lean_object* x_75; lean_object* x_76; lean_object* x_77; lean_object* x_78; lean_object* x_79; lean_object* x_80; lean_object* x_81; lean_object* x_82; 
-lean_inc(x_35);
-x_71 = lean_alloc_ctor(2, 1, 0);
-lean_ctor_set(x_71, 0, x_35);
-x_72 = l_Array_foldlMUnsafe_fold___at_Lean_withNestedTraces___spec__5___closed__1;
-x_73 = lean_alloc_ctor(10, 2, 0);
-lean_ctor_set(x_73, 0, x_72);
-lean_ctor_set(x_73, 1, x_71);
-x_74 = l_Lean_Meta_isLevelDefEqAux___closed__6;
-x_75 = lean_alloc_ctor(10, 2, 0);
-lean_ctor_set(x_75, 0, x_73);
-lean_ctor_set(x_75, 1, x_74);
-lean_inc(x_46);
-x_76 = lean_alloc_ctor(2, 1, 0);
-lean_ctor_set(x_76, 0, x_46);
-x_77 = lean_alloc_ctor(10, 2, 0);
-lean_ctor_set(x_77, 0, x_75);
-lean_ctor_set(x_77, 1, x_76);
-x_78 = lean_alloc_ctor(10, 2, 0);
-lean_ctor_set(x_78, 0, x_77);
-lean_ctor_set(x_78, 1, x_72);
-x_79 = l___private_Lean_Elab_App_0__Lean_Elab_Term_ElabAppArgs_propagateExpectedType___closed__3;
-x_80 = l_Lean_addTrace___at___private_Lean_Elab_App_0__Lean_Elab_Term_ElabAppArgs_propagateExpectedType___spec__6(x_79, x_78, x_1, x_2, x_3, x_4, x_5, x_6, x_7, x_59);
-x_81 = lean_ctor_get(x_80, 1);
-lean_inc(x_81);
-lean_dec(x_80);
-x_82 = l_Lean_Meta_isExprDefEq___at___private_Lean_Elab_App_0__Lean_Elab_Term_ElabAppArgs_propagateExpectedType___spec__3(x_35, x_46, x_1, x_2, x_3, x_4, x_5, x_6, x_7, x_81);
-lean_dec(x_3);
-lean_dec(x_2);
+uint8_t x_62; lean_object* x_63; uint8_t x_64; 
+x_62 = 1;
+lean_ctor_set_uint8(x_59, sizeof(void*)*9 + 2, x_62);
+x_63 = lean_st_ref_set(x_1, x_59, x_60);
 lean_dec(x_1);
-if (lean_obj_tag(x_82) == 0)
+x_64 = !lean_is_exclusive(x_63);
+if (x_64 == 0)
 {
-uint8_t x_83; 
-x_83 = !lean_is_exclusive(x_82);
-if (x_83 == 0)
-{
-lean_object* x_84; lean_object* x_85; 
-x_84 = lean_ctor_get(x_82, 0);
-lean_dec(x_84);
-x_85 = lean_box(0);
-lean_ctor_set(x_82, 0, x_85);
-return x_82;
+lean_object* x_65; lean_object* x_66; 
+x_65 = lean_ctor_get(x_63, 0);
+lean_dec(x_65);
+x_66 = lean_box(0);
+lean_ctor_set(x_63, 0, x_66);
+return x_63;
 }
 else
 {
-lean_object* x_86; lean_object* x_87; lean_object* x_88; 
-x_86 = lean_ctor_get(x_82, 1);
-lean_inc(x_86);
-lean_dec(x_82);
-x_87 = lean_box(0);
-x_88 = lean_alloc_ctor(0, 2, 0);
-lean_ctor_set(x_88, 0, x_87);
-lean_ctor_set(x_88, 1, x_86);
-return x_88;
+lean_object* x_67; lean_object* x_68; lean_object* x_69; 
+x_67 = lean_ctor_get(x_63, 1);
+lean_inc(x_67);
+lean_dec(x_63);
+x_68 = lean_box(0);
+x_69 = lean_alloc_ctor(0, 2, 0);
+lean_ctor_set(x_69, 0, x_68);
+lean_ctor_set(x_69, 1, x_67);
+return x_69;
 }
 }
 else
 {
-uint8_t x_89; 
-x_89 = !lean_is_exclusive(x_82);
-if (x_89 == 0)
-{
-return x_82;
+uint8_t x_70; lean_object* x_71; lean_object* x_72; lean_object* x_73; lean_object* x_74; uint8_t x_75; lean_object* x_76; lean_object* x_77; lean_object* x_78; lean_object* x_79; lean_object* x_80; uint8_t x_81; lean_object* x_82; lean_object* x_83; lean_object* x_84; lean_object* x_85; lean_object* x_86; lean_object* x_87; 
+x_70 = lean_ctor_get_uint8(x_59, sizeof(void*)*9);
+x_71 = lean_ctor_get(x_59, 0);
+x_72 = lean_ctor_get(x_59, 1);
+x_73 = lean_ctor_get(x_59, 2);
+x_74 = lean_ctor_get(x_59, 3);
+x_75 = lean_ctor_get_uint8(x_59, sizeof(void*)*9 + 1);
+x_76 = lean_ctor_get(x_59, 4);
+x_77 = lean_ctor_get(x_59, 5);
+x_78 = lean_ctor_get(x_59, 6);
+x_79 = lean_ctor_get(x_59, 7);
+x_80 = lean_ctor_get(x_59, 8);
+lean_inc(x_80);
+lean_inc(x_79);
+lean_inc(x_78);
+lean_inc(x_77);
+lean_inc(x_76);
+lean_inc(x_74);
+lean_inc(x_73);
+lean_inc(x_72);
+lean_inc(x_71);
+lean_dec(x_59);
+x_81 = 1;
+x_82 = lean_alloc_ctor(0, 9, 3);
+lean_ctor_set(x_82, 0, x_71);
+lean_ctor_set(x_82, 1, x_72);
+lean_ctor_set(x_82, 2, x_73);
+lean_ctor_set(x_82, 3, x_74);
+lean_ctor_set(x_82, 4, x_76);
+lean_ctor_set(x_82, 5, x_77);
+lean_ctor_set(x_82, 6, x_78);
+lean_ctor_set(x_82, 7, x_79);
+lean_ctor_set(x_82, 8, x_80);
+lean_ctor_set_uint8(x_82, sizeof(void*)*9, x_70);
+lean_ctor_set_uint8(x_82, sizeof(void*)*9 + 1, x_75);
+lean_ctor_set_uint8(x_82, sizeof(void*)*9 + 2, x_81);
+x_83 = lean_st_ref_set(x_1, x_82, x_60);
+lean_dec(x_1);
+x_84 = lean_ctor_get(x_83, 1);
+lean_inc(x_84);
+if (lean_is_exclusive(x_83)) {
+ lean_ctor_release(x_83, 0);
+ lean_ctor_release(x_83, 1);
+ x_85 = x_83;
+} else {
+ lean_dec_ref(x_83);
+ x_85 = lean_box(0);
+}
+x_86 = lean_box(0);
+if (lean_is_scalar(x_85)) {
+ x_87 = lean_alloc_ctor(0, 2, 0);
+} else {
+ x_87 = x_85;
+}
+lean_ctor_set(x_87, 0, x_86);
+lean_ctor_set(x_87, 1, x_84);
+return x_87;
+}
+}
 }
 else
 {
-lean_object* x_90; lean_object* x_91; lean_object* x_92; 
-x_90 = lean_ctor_get(x_82, 0);
-x_91 = lean_ctor_get(x_82, 1);
-lean_inc(x_91);
+uint8_t x_88; 
+lean_dec(x_1);
+x_88 = !lean_is_exclusive(x_48);
+if (x_88 == 0)
+{
+return x_48;
+}
+else
+{
+lean_object* x_89; lean_object* x_90; lean_object* x_91; 
+x_89 = lean_ctor_get(x_48, 0);
+x_90 = lean_ctor_get(x_48, 1);
 lean_inc(x_90);
-lean_dec(x_82);
-x_92 = lean_alloc_ctor(1, 2, 0);
-lean_ctor_set(x_92, 0, x_90);
-lean_ctor_set(x_92, 1, x_91);
-return x_92;
+lean_inc(x_89);
+lean_dec(x_48);
+x_91 = lean_alloc_ctor(1, 2, 0);
+lean_ctor_set(x_91, 0, x_89);
+lean_ctor_set(x_91, 1, x_90);
+return x_91;
 }
 }
 }
-}
+block_106:
+{
+if (x_93 == 0)
+{
+x_47 = x_94;
+goto block_92;
 }
 else
 {
-lean_object* x_108; lean_object* x_109; uint8_t x_110; lean_object* x_111; uint8_t x_142; 
-x_108 = lean_ctor_get(x_54, 0);
-x_109 = lean_ctor_get(x_54, 1);
-lean_inc(x_109);
-lean_inc(x_108);
-lean_dec(x_54);
-x_142 = lean_unbox(x_108);
-lean_dec(x_108);
-if (x_142 == 0)
-{
-lean_object* x_143; lean_object* x_144; lean_object* x_145; uint8_t x_146; 
-x_143 = lean_st_ref_get(x_7, x_109);
-x_144 = lean_ctor_get(x_143, 0);
-lean_inc(x_144);
-x_145 = lean_ctor_get(x_144, 3);
-lean_inc(x_145);
-lean_dec(x_144);
-x_146 = lean_ctor_get_uint8(x_145, sizeof(void*)*1);
-lean_dec(x_145);
-if (x_146 == 0)
-{
-lean_object* x_147; uint8_t x_148; 
-x_147 = lean_ctor_get(x_143, 1);
-lean_inc(x_147);
-lean_dec(x_143);
-x_148 = 0;
-x_110 = x_148;
-x_111 = x_147;
-goto block_141;
-}
-else
-{
-lean_object* x_149; lean_object* x_150; lean_object* x_151; lean_object* x_152; lean_object* x_153; uint8_t x_154; 
-x_149 = lean_ctor_get(x_143, 1);
-lean_inc(x_149);
-lean_dec(x_143);
-x_150 = l___private_Lean_Elab_App_0__Lean_Elab_Term_ElabAppArgs_propagateExpectedType___closed__3;
-x_151 = l___private_Lean_Util_Trace_0__Lean_checkTraceOptionM___at___private_Lean_Elab_App_0__Lean_Elab_Term_ElabAppArgs_propagateExpectedType___spec__7(x_150, x_1, x_2, x_3, x_4, x_5, x_6, x_7, x_149);
-x_152 = lean_ctor_get(x_151, 0);
-lean_inc(x_152);
-x_153 = lean_ctor_get(x_151, 1);
-lean_inc(x_153);
-lean_dec(x_151);
-x_154 = lean_unbox(x_152);
-lean_dec(x_152);
-x_110 = x_154;
-x_111 = x_153;
-goto block_141;
-}
-}
-else
-{
-lean_object* x_155; lean_object* x_156; 
-lean_dec(x_46);
-lean_dec(x_35);
-lean_dec(x_7);
-lean_dec(x_6);
-lean_dec(x_5);
-lean_dec(x_4);
-lean_dec(x_3);
-lean_dec(x_2);
-lean_dec(x_1);
-x_155 = lean_box(0);
-x_156 = lean_alloc_ctor(0, 2, 0);
-lean_ctor_set(x_156, 0, x_155);
-lean_ctor_set(x_156, 1, x_109);
-return x_156;
-}
-block_141:
-{
-if (x_110 == 0)
-{
-lean_object* x_112; 
-x_112 = l_Lean_Meta_isExprDefEq___at___private_Lean_Elab_App_0__Lean_Elab_Term_ElabAppArgs_propagateExpectedType___spec__3(x_35, x_46, x_1, x_2, x_3, x_4, x_5, x_6, x_7, x_111);
-lean_dec(x_3);
-lean_dec(x_2);
-lean_dec(x_1);
-if (lean_obj_tag(x_112) == 0)
-{
-lean_object* x_113; lean_object* x_114; lean_object* x_115; lean_object* x_116; 
-x_113 = lean_ctor_get(x_112, 1);
-lean_inc(x_113);
-if (lean_is_exclusive(x_112)) {
- lean_ctor_release(x_112, 0);
- lean_ctor_release(x_112, 1);
- x_114 = x_112;
-} else {
- lean_dec_ref(x_112);
- x_114 = lean_box(0);
-}
-x_115 = lean_box(0);
-if (lean_is_scalar(x_114)) {
- x_116 = lean_alloc_ctor(0, 2, 0);
-} else {
- x_116 = x_114;
-}
-lean_ctor_set(x_116, 0, x_115);
-lean_ctor_set(x_116, 1, x_113);
-return x_116;
-}
-else
-{
-lean_object* x_117; lean_object* x_118; lean_object* x_119; lean_object* x_120; 
-x_117 = lean_ctor_get(x_112, 0);
-lean_inc(x_117);
-x_118 = lean_ctor_get(x_112, 1);
-lean_inc(x_118);
-if (lean_is_exclusive(x_112)) {
- lean_ctor_release(x_112, 0);
- lean_ctor_release(x_112, 1);
- x_119 = x_112;
-} else {
- lean_dec_ref(x_112);
- x_119 = lean_box(0);
-}
-if (lean_is_scalar(x_119)) {
- x_120 = lean_alloc_ctor(1, 2, 0);
-} else {
- x_120 = x_119;
-}
-lean_ctor_set(x_120, 0, x_117);
-lean_ctor_set(x_120, 1, x_118);
-return x_120;
-}
-}
-else
-{
-lean_object* x_121; lean_object* x_122; lean_object* x_123; lean_object* x_124; lean_object* x_125; lean_object* x_126; lean_object* x_127; lean_object* x_128; lean_object* x_129; lean_object* x_130; lean_object* x_131; lean_object* x_132; 
+lean_object* x_95; lean_object* x_96; lean_object* x_97; lean_object* x_98; lean_object* x_99; lean_object* x_100; lean_object* x_101; lean_object* x_102; lean_object* x_103; lean_object* x_104; lean_object* x_105; 
+lean_inc(x_24);
+x_95 = lean_alloc_ctor(2, 1, 0);
+lean_ctor_set(x_95, 0, x_24);
+x_96 = l_Array_foldlMUnsafe_fold___at_Lean_withNestedTraces___spec__5___closed__1;
+x_97 = lean_alloc_ctor(10, 2, 0);
+lean_ctor_set(x_97, 0, x_96);
+lean_ctor_set(x_97, 1, x_95);
+x_98 = l_Lean_Meta_isLevelDefEqAux___closed__6;
+x_99 = lean_alloc_ctor(10, 2, 0);
+lean_ctor_set(x_99, 0, x_97);
+lean_ctor_set(x_99, 1, x_98);
 lean_inc(x_35);
-x_121 = lean_alloc_ctor(2, 1, 0);
-lean_ctor_set(x_121, 0, x_35);
-x_122 = l_Array_foldlMUnsafe_fold___at_Lean_withNestedTraces___spec__5___closed__1;
-x_123 = lean_alloc_ctor(10, 2, 0);
-lean_ctor_set(x_123, 0, x_122);
-lean_ctor_set(x_123, 1, x_121);
-x_124 = l_Lean_Meta_isLevelDefEqAux___closed__6;
-x_125 = lean_alloc_ctor(10, 2, 0);
-lean_ctor_set(x_125, 0, x_123);
-lean_ctor_set(x_125, 1, x_124);
-lean_inc(x_46);
-x_126 = lean_alloc_ctor(2, 1, 0);
-lean_ctor_set(x_126, 0, x_46);
-x_127 = lean_alloc_ctor(10, 2, 0);
-lean_ctor_set(x_127, 0, x_125);
-lean_ctor_set(x_127, 1, x_126);
-x_128 = lean_alloc_ctor(10, 2, 0);
-lean_ctor_set(x_128, 0, x_127);
-lean_ctor_set(x_128, 1, x_122);
-x_129 = l___private_Lean_Elab_App_0__Lean_Elab_Term_ElabAppArgs_propagateExpectedType___closed__3;
-x_130 = l_Lean_addTrace___at___private_Lean_Elab_App_0__Lean_Elab_Term_ElabAppArgs_propagateExpectedType___spec__6(x_129, x_128, x_1, x_2, x_3, x_4, x_5, x_6, x_7, x_111);
-x_131 = lean_ctor_get(x_130, 1);
-lean_inc(x_131);
-lean_dec(x_130);
-x_132 = l_Lean_Meta_isExprDefEq___at___private_Lean_Elab_App_0__Lean_Elab_Term_ElabAppArgs_propagateExpectedType___spec__3(x_35, x_46, x_1, x_2, x_3, x_4, x_5, x_6, x_7, x_131);
-lean_dec(x_3);
-lean_dec(x_2);
-lean_dec(x_1);
-if (lean_obj_tag(x_132) == 0)
-{
-lean_object* x_133; lean_object* x_134; lean_object* x_135; lean_object* x_136; 
-x_133 = lean_ctor_get(x_132, 1);
-lean_inc(x_133);
-if (lean_is_exclusive(x_132)) {
- lean_ctor_release(x_132, 0);
- lean_ctor_release(x_132, 1);
- x_134 = x_132;
-} else {
- lean_dec_ref(x_132);
- x_134 = lean_box(0);
-}
-x_135 = lean_box(0);
-if (lean_is_scalar(x_134)) {
- x_136 = lean_alloc_ctor(0, 2, 0);
-} else {
- x_136 = x_134;
-}
-lean_ctor_set(x_136, 0, x_135);
-lean_ctor_set(x_136, 1, x_133);
-return x_136;
-}
-else
-{
-lean_object* x_137; lean_object* x_138; lean_object* x_139; lean_object* x_140; 
-x_137 = lean_ctor_get(x_132, 0);
-lean_inc(x_137);
-x_138 = lean_ctor_get(x_132, 1);
-lean_inc(x_138);
-if (lean_is_exclusive(x_132)) {
- lean_ctor_release(x_132, 0);
- lean_ctor_release(x_132, 1);
- x_139 = x_132;
-} else {
- lean_dec_ref(x_132);
- x_139 = lean_box(0);
-}
-if (lean_is_scalar(x_139)) {
- x_140 = lean_alloc_ctor(1, 2, 0);
-} else {
- x_140 = x_139;
-}
-lean_ctor_set(x_140, 0, x_137);
-lean_ctor_set(x_140, 1, x_138);
-return x_140;
-}
-}
+x_100 = lean_alloc_ctor(2, 1, 0);
+lean_ctor_set(x_100, 0, x_35);
+x_101 = lean_alloc_ctor(10, 2, 0);
+lean_ctor_set(x_101, 0, x_99);
+lean_ctor_set(x_101, 1, x_100);
+x_102 = lean_alloc_ctor(10, 2, 0);
+lean_ctor_set(x_102, 0, x_101);
+lean_ctor_set(x_102, 1, x_96);
+x_103 = l___private_Lean_Elab_App_0__Lean_Elab_Term_ElabAppArgs_propagateExpectedType___closed__3;
+x_104 = l_Lean_addTrace___at___private_Lean_Elab_App_0__Lean_Elab_Term_ElabAppArgs_propagateExpectedType___spec__6(x_103, x_102, x_1, x_2, x_3, x_4, x_5, x_6, x_7, x_94);
+x_105 = lean_ctor_get(x_104, 1);
+lean_inc(x_105);
+lean_dec(x_104);
+x_47 = x_105;
+goto block_92;
 }
 }
 }
 else
 {
-uint8_t x_157; 
-lean_dec(x_46);
-lean_dec(x_35);
-lean_dec(x_7);
-lean_dec(x_6);
-lean_dec(x_5);
-lean_dec(x_4);
-lean_dec(x_3);
-lean_dec(x_2);
-lean_dec(x_1);
-x_157 = !lean_is_exclusive(x_54);
-if (x_157 == 0)
+lean_object* x_121; lean_object* x_122; lean_object* x_123; uint8_t x_159; lean_object* x_160; uint8_t x_173; 
+x_121 = lean_ctor_get(x_43, 0);
+x_122 = lean_ctor_get(x_43, 1);
+lean_inc(x_122);
+lean_inc(x_121);
+lean_dec(x_43);
+x_173 = lean_unbox(x_121);
+lean_dec(x_121);
+if (x_173 == 0)
 {
-return x_54;
+lean_object* x_174; lean_object* x_175; lean_object* x_176; uint8_t x_177; 
+x_174 = lean_st_ref_get(x_7, x_122);
+x_175 = lean_ctor_get(x_174, 0);
+lean_inc(x_175);
+x_176 = lean_ctor_get(x_175, 3);
+lean_inc(x_176);
+lean_dec(x_175);
+x_177 = lean_ctor_get_uint8(x_176, sizeof(void*)*1);
+lean_dec(x_176);
+if (x_177 == 0)
+{
+lean_object* x_178; uint8_t x_179; 
+x_178 = lean_ctor_get(x_174, 1);
+lean_inc(x_178);
+lean_dec(x_174);
+x_179 = 0;
+x_159 = x_179;
+x_160 = x_178;
+goto block_172;
 }
 else
 {
-lean_object* x_158; lean_object* x_159; lean_object* x_160; 
-x_158 = lean_ctor_get(x_54, 0);
-x_159 = lean_ctor_get(x_54, 1);
-lean_inc(x_159);
-lean_inc(x_158);
-lean_dec(x_54);
-x_160 = lean_alloc_ctor(1, 2, 0);
-lean_ctor_set(x_160, 0, x_158);
-lean_ctor_set(x_160, 1, x_159);
-return x_160;
-}
-}
-}
-else
-{
-lean_object* x_161; lean_object* x_162; 
-lean_dec(x_52);
-lean_dec(x_46);
-lean_dec(x_35);
-lean_dec(x_7);
-lean_dec(x_6);
-lean_dec(x_5);
-lean_dec(x_4);
-lean_dec(x_3);
-lean_dec(x_2);
-lean_dec(x_1);
-x_161 = lean_box(0);
-if (lean_is_scalar(x_34)) {
- x_162 = lean_alloc_ctor(0, 2, 0);
-} else {
- x_162 = x_34;
-}
-lean_ctor_set(x_162, 0, x_161);
-lean_ctor_set(x_162, 1, x_40);
-return x_162;
-}
-}
-}
-else
-{
-lean_object* x_163; lean_object* x_164; 
-lean_dec(x_46);
-lean_dec(x_35);
-lean_dec(x_18);
-lean_dec(x_11);
-lean_dec(x_7);
-lean_dec(x_6);
-lean_dec(x_5);
-lean_dec(x_4);
-lean_dec(x_3);
-lean_dec(x_2);
-lean_dec(x_1);
-x_163 = lean_box(0);
-if (lean_is_scalar(x_34)) {
- x_164 = lean_alloc_ctor(0, 2, 0);
-} else {
- x_164 = x_34;
-}
-lean_ctor_set(x_164, 0, x_163);
-lean_ctor_set(x_164, 1, x_40);
-return x_164;
-}
-}
-}
-block_188:
-{
-if (x_166 == 0)
-{
-lean_dec(x_14);
-x_40 = x_167;
-goto block_165;
-}
-else
-{
-lean_object* x_168; lean_object* x_169; lean_object* x_170; lean_object* x_171; lean_object* x_172; lean_object* x_173; lean_object* x_174; lean_object* x_175; lean_object* x_176; lean_object* x_177; lean_object* x_178; lean_object* x_179; lean_object* x_180; lean_object* x_181; lean_object* x_182; lean_object* x_183; lean_object* x_184; lean_object* x_185; lean_object* x_186; lean_object* x_187; 
-x_168 = lean_array_get_size(x_14);
-lean_dec(x_14);
-x_169 = l_Lean_fmt___at_Lean_Position_instToFormatPosition___spec__1(x_168);
-x_170 = lean_alloc_ctor(0, 1, 0);
-lean_ctor_set(x_170, 0, x_169);
-x_171 = l___private_Lean_Elab_App_0__Lean_Elab_Term_ElabAppArgs_propagateExpectedType___closed__5;
-x_172 = lean_alloc_ctor(10, 2, 0);
-lean_ctor_set(x_172, 0, x_171);
-lean_ctor_set(x_172, 1, x_170);
-x_173 = l___private_Lean_Elab_App_0__Lean_Elab_Term_ElabAppArgs_propagateExpectedType___closed__7;
-x_174 = lean_alloc_ctor(10, 2, 0);
-lean_ctor_set(x_174, 0, x_172);
-lean_ctor_set(x_174, 1, x_173);
-lean_inc(x_39);
-x_175 = l_Lean_fmt___at_Lean_Position_instToFormatPosition___spec__1(x_39);
-x_176 = lean_alloc_ctor(0, 1, 0);
-lean_ctor_set(x_176, 0, x_175);
-x_177 = lean_alloc_ctor(10, 2, 0);
-lean_ctor_set(x_177, 0, x_174);
-lean_ctor_set(x_177, 1, x_176);
-x_178 = l___private_Lean_Elab_App_0__Lean_Elab_Term_ElabAppArgs_propagateExpectedType___closed__9;
-x_179 = lean_alloc_ctor(10, 2, 0);
-lean_ctor_set(x_179, 0, x_177);
-lean_ctor_set(x_179, 1, x_178);
-x_180 = lean_ctor_get(x_11, 1);
+lean_object* x_180; lean_object* x_181; lean_object* x_182; lean_object* x_183; lean_object* x_184; uint8_t x_185; 
+x_180 = lean_ctor_get(x_174, 1);
 lean_inc(x_180);
-x_181 = lean_alloc_ctor(2, 1, 0);
-lean_ctor_set(x_181, 0, x_180);
-x_182 = lean_alloc_ctor(10, 2, 0);
-lean_ctor_set(x_182, 0, x_179);
-lean_ctor_set(x_182, 1, x_181);
-x_183 = l_Array_foldlMUnsafe_fold___at_Lean_withNestedTraces___spec__5___closed__1;
-x_184 = lean_alloc_ctor(10, 2, 0);
-lean_ctor_set(x_184, 0, x_182);
-lean_ctor_set(x_184, 1, x_183);
-x_185 = l___private_Lean_Elab_App_0__Lean_Elab_Term_ElabAppArgs_propagateExpectedType___closed__3;
-x_186 = l_Lean_addTrace___at___private_Lean_Elab_App_0__Lean_Elab_Term_ElabAppArgs_propagateExpectedType___spec__6(x_185, x_184, x_1, x_2, x_3, x_4, x_5, x_6, x_7, x_167);
-x_187 = lean_ctor_get(x_186, 1);
-lean_inc(x_187);
-lean_dec(x_186);
-x_40 = x_187;
-goto block_165;
-}
+lean_dec(x_174);
+x_181 = l___private_Lean_Elab_App_0__Lean_Elab_Term_ElabAppArgs_propagateExpectedType___closed__3;
+x_182 = l___private_Lean_Util_Trace_0__Lean_checkTraceOptionM___at___private_Lean_Elab_App_0__Lean_Elab_Term_ElabAppArgs_propagateExpectedType___spec__7(x_181, x_1, x_2, x_3, x_4, x_5, x_6, x_7, x_180);
+x_183 = lean_ctor_get(x_182, 0);
+lean_inc(x_183);
+x_184 = lean_ctor_get(x_182, 1);
+lean_inc(x_184);
+lean_dec(x_182);
+x_185 = lean_unbox(x_183);
+lean_dec(x_183);
+x_159 = x_185;
+x_160 = x_184;
+goto block_172;
 }
 }
 else
 {
-lean_object* x_201; lean_object* x_202; 
+lean_object* x_186; lean_object* x_187; 
 lean_dec(x_35);
-lean_dec(x_18);
-lean_dec(x_14);
-lean_dec(x_11);
+lean_dec(x_24);
 lean_dec(x_7);
 lean_dec(x_6);
 lean_dec(x_5);
@@ -14134,611 +13878,509 @@ lean_dec(x_4);
 lean_dec(x_3);
 lean_dec(x_2);
 lean_dec(x_1);
-x_201 = lean_box(0);
-if (lean_is_scalar(x_34)) {
- x_202 = lean_alloc_ctor(0, 2, 0);
-} else {
- x_202 = x_34;
+x_186 = lean_box(0);
+x_187 = lean_alloc_ctor(0, 2, 0);
+lean_ctor_set(x_187, 0, x_186);
+lean_ctor_set(x_187, 1, x_122);
+return x_187;
 }
-lean_ctor_set(x_202, 0, x_201);
-lean_ctor_set(x_202, 1, x_33);
-return x_202;
+block_158:
+{
+lean_object* x_124; 
+x_124 = l_Lean_Meta_isExprDefEq___at___private_Lean_Elab_App_0__Lean_Elab_Term_ElabAppArgs_propagateExpectedType___spec__3(x_24, x_35, x_1, x_2, x_3, x_4, x_5, x_6, x_7, x_123);
+lean_dec(x_3);
+lean_dec(x_2);
+if (lean_obj_tag(x_124) == 0)
+{
+lean_object* x_125; uint8_t x_126; 
+x_125 = lean_ctor_get(x_124, 0);
+lean_inc(x_125);
+x_126 = lean_unbox(x_125);
+lean_dec(x_125);
+if (x_126 == 0)
+{
+lean_object* x_127; lean_object* x_128; lean_object* x_129; lean_object* x_130; 
+lean_dec(x_1);
+x_127 = lean_ctor_get(x_124, 1);
+lean_inc(x_127);
+if (lean_is_exclusive(x_124)) {
+ lean_ctor_release(x_124, 0);
+ lean_ctor_release(x_124, 1);
+ x_128 = x_124;
+} else {
+ lean_dec_ref(x_124);
+ x_128 = lean_box(0);
+}
+x_129 = lean_box(0);
+if (lean_is_scalar(x_128)) {
+ x_130 = lean_alloc_ctor(0, 2, 0);
+} else {
+ x_130 = x_128;
+}
+lean_ctor_set(x_130, 0, x_129);
+lean_ctor_set(x_130, 1, x_127);
+return x_130;
+}
+else
+{
+lean_object* x_131; lean_object* x_132; lean_object* x_133; lean_object* x_134; uint8_t x_135; lean_object* x_136; lean_object* x_137; lean_object* x_138; lean_object* x_139; uint8_t x_140; lean_object* x_141; lean_object* x_142; lean_object* x_143; lean_object* x_144; lean_object* x_145; lean_object* x_146; uint8_t x_147; lean_object* x_148; lean_object* x_149; lean_object* x_150; lean_object* x_151; lean_object* x_152; lean_object* x_153; 
+x_131 = lean_ctor_get(x_124, 1);
+lean_inc(x_131);
+lean_dec(x_124);
+x_132 = lean_st_ref_take(x_1, x_131);
+x_133 = lean_ctor_get(x_132, 0);
+lean_inc(x_133);
+x_134 = lean_ctor_get(x_132, 1);
+lean_inc(x_134);
+lean_dec(x_132);
+x_135 = lean_ctor_get_uint8(x_133, sizeof(void*)*9);
+x_136 = lean_ctor_get(x_133, 0);
+lean_inc(x_136);
+x_137 = lean_ctor_get(x_133, 1);
+lean_inc(x_137);
+x_138 = lean_ctor_get(x_133, 2);
+lean_inc(x_138);
+x_139 = lean_ctor_get(x_133, 3);
+lean_inc(x_139);
+x_140 = lean_ctor_get_uint8(x_133, sizeof(void*)*9 + 1);
+x_141 = lean_ctor_get(x_133, 4);
+lean_inc(x_141);
+x_142 = lean_ctor_get(x_133, 5);
+lean_inc(x_142);
+x_143 = lean_ctor_get(x_133, 6);
+lean_inc(x_143);
+x_144 = lean_ctor_get(x_133, 7);
+lean_inc(x_144);
+x_145 = lean_ctor_get(x_133, 8);
+lean_inc(x_145);
+if (lean_is_exclusive(x_133)) {
+ lean_ctor_release(x_133, 0);
+ lean_ctor_release(x_133, 1);
+ lean_ctor_release(x_133, 2);
+ lean_ctor_release(x_133, 3);
+ lean_ctor_release(x_133, 4);
+ lean_ctor_release(x_133, 5);
+ lean_ctor_release(x_133, 6);
+ lean_ctor_release(x_133, 7);
+ lean_ctor_release(x_133, 8);
+ x_146 = x_133;
+} else {
+ lean_dec_ref(x_133);
+ x_146 = lean_box(0);
+}
+x_147 = 1;
+if (lean_is_scalar(x_146)) {
+ x_148 = lean_alloc_ctor(0, 9, 3);
+} else {
+ x_148 = x_146;
+}
+lean_ctor_set(x_148, 0, x_136);
+lean_ctor_set(x_148, 1, x_137);
+lean_ctor_set(x_148, 2, x_138);
+lean_ctor_set(x_148, 3, x_139);
+lean_ctor_set(x_148, 4, x_141);
+lean_ctor_set(x_148, 5, x_142);
+lean_ctor_set(x_148, 6, x_143);
+lean_ctor_set(x_148, 7, x_144);
+lean_ctor_set(x_148, 8, x_145);
+lean_ctor_set_uint8(x_148, sizeof(void*)*9, x_135);
+lean_ctor_set_uint8(x_148, sizeof(void*)*9 + 1, x_140);
+lean_ctor_set_uint8(x_148, sizeof(void*)*9 + 2, x_147);
+x_149 = lean_st_ref_set(x_1, x_148, x_134);
+lean_dec(x_1);
+x_150 = lean_ctor_get(x_149, 1);
+lean_inc(x_150);
+if (lean_is_exclusive(x_149)) {
+ lean_ctor_release(x_149, 0);
+ lean_ctor_release(x_149, 1);
+ x_151 = x_149;
+} else {
+ lean_dec_ref(x_149);
+ x_151 = lean_box(0);
+}
+x_152 = lean_box(0);
+if (lean_is_scalar(x_151)) {
+ x_153 = lean_alloc_ctor(0, 2, 0);
+} else {
+ x_153 = x_151;
+}
+lean_ctor_set(x_153, 0, x_152);
+lean_ctor_set(x_153, 1, x_150);
+return x_153;
+}
+}
+else
+{
+lean_object* x_154; lean_object* x_155; lean_object* x_156; lean_object* x_157; 
+lean_dec(x_1);
+x_154 = lean_ctor_get(x_124, 0);
+lean_inc(x_154);
+x_155 = lean_ctor_get(x_124, 1);
+lean_inc(x_155);
+if (lean_is_exclusive(x_124)) {
+ lean_ctor_release(x_124, 0);
+ lean_ctor_release(x_124, 1);
+ x_156 = x_124;
+} else {
+ lean_dec_ref(x_124);
+ x_156 = lean_box(0);
+}
+if (lean_is_scalar(x_156)) {
+ x_157 = lean_alloc_ctor(1, 2, 0);
+} else {
+ x_157 = x_156;
+}
+lean_ctor_set(x_157, 0, x_154);
+lean_ctor_set(x_157, 1, x_155);
+return x_157;
+}
+}
+block_172:
+{
+if (x_159 == 0)
+{
+x_123 = x_160;
+goto block_158;
+}
+else
+{
+lean_object* x_161; lean_object* x_162; lean_object* x_163; lean_object* x_164; lean_object* x_165; lean_object* x_166; lean_object* x_167; lean_object* x_168; lean_object* x_169; lean_object* x_170; lean_object* x_171; 
+lean_inc(x_24);
+x_161 = lean_alloc_ctor(2, 1, 0);
+lean_ctor_set(x_161, 0, x_24);
+x_162 = l_Array_foldlMUnsafe_fold___at_Lean_withNestedTraces___spec__5___closed__1;
+x_163 = lean_alloc_ctor(10, 2, 0);
+lean_ctor_set(x_163, 0, x_162);
+lean_ctor_set(x_163, 1, x_161);
+x_164 = l_Lean_Meta_isLevelDefEqAux___closed__6;
+x_165 = lean_alloc_ctor(10, 2, 0);
+lean_ctor_set(x_165, 0, x_163);
+lean_ctor_set(x_165, 1, x_164);
+lean_inc(x_35);
+x_166 = lean_alloc_ctor(2, 1, 0);
+lean_ctor_set(x_166, 0, x_35);
+x_167 = lean_alloc_ctor(10, 2, 0);
+lean_ctor_set(x_167, 0, x_165);
+lean_ctor_set(x_167, 1, x_166);
+x_168 = lean_alloc_ctor(10, 2, 0);
+lean_ctor_set(x_168, 0, x_167);
+lean_ctor_set(x_168, 1, x_162);
+x_169 = l___private_Lean_Elab_App_0__Lean_Elab_Term_ElabAppArgs_propagateExpectedType___closed__3;
+x_170 = l_Lean_addTrace___at___private_Lean_Elab_App_0__Lean_Elab_Term_ElabAppArgs_propagateExpectedType___spec__6(x_169, x_168, x_1, x_2, x_3, x_4, x_5, x_6, x_7, x_160);
+x_171 = lean_ctor_get(x_170, 1);
+lean_inc(x_171);
+lean_dec(x_170);
+x_123 = x_171;
+goto block_158;
+}
 }
 }
 }
 else
 {
-uint8_t x_203; lean_object* x_204; lean_object* x_205; lean_object* x_206; lean_object* x_207; uint8_t x_208; lean_object* x_209; lean_object* x_210; lean_object* x_211; lean_object* x_212; lean_object* x_213; uint8_t x_214; lean_object* x_215; lean_object* x_216; lean_object* x_217; 
-x_203 = lean_ctor_get_uint8(x_21, sizeof(void*)*9);
-x_204 = lean_ctor_get(x_21, 0);
-x_205 = lean_ctor_get(x_21, 1);
-x_206 = lean_ctor_get(x_21, 2);
-x_207 = lean_ctor_get(x_21, 3);
-x_208 = lean_ctor_get_uint8(x_21, sizeof(void*)*9 + 1);
-x_209 = lean_ctor_get(x_21, 4);
-x_210 = lean_ctor_get(x_21, 5);
-x_211 = lean_ctor_get(x_21, 6);
-x_212 = lean_ctor_get(x_21, 7);
-x_213 = lean_ctor_get(x_21, 8);
-lean_inc(x_213);
-lean_inc(x_212);
+uint8_t x_188; 
+lean_dec(x_35);
+lean_dec(x_24);
+lean_dec(x_7);
+lean_dec(x_6);
+lean_dec(x_5);
+lean_dec(x_4);
+lean_dec(x_3);
+lean_dec(x_2);
+lean_dec(x_1);
+x_188 = !lean_is_exclusive(x_43);
+if (x_188 == 0)
+{
+return x_43;
+}
+else
+{
+lean_object* x_189; lean_object* x_190; lean_object* x_191; 
+x_189 = lean_ctor_get(x_43, 0);
+x_190 = lean_ctor_get(x_43, 1);
+lean_inc(x_190);
+lean_inc(x_189);
+lean_dec(x_43);
+x_191 = lean_alloc_ctor(1, 2, 0);
+lean_ctor_set(x_191, 0, x_189);
+lean_ctor_set(x_191, 1, x_190);
+return x_191;
+}
+}
+}
+else
+{
+lean_object* x_192; lean_object* x_193; 
+lean_dec(x_41);
+lean_dec(x_35);
+lean_dec(x_24);
+lean_dec(x_7);
+lean_dec(x_6);
+lean_dec(x_5);
+lean_dec(x_4);
+lean_dec(x_3);
+lean_dec(x_2);
+lean_dec(x_1);
+x_192 = lean_box(0);
+if (lean_is_scalar(x_12)) {
+ x_193 = lean_alloc_ctor(0, 2, 0);
+} else {
+ x_193 = x_12;
+}
+lean_ctor_set(x_193, 0, x_192);
+lean_ctor_set(x_193, 1, x_29);
+return x_193;
+}
+}
+}
+else
+{
+lean_object* x_194; lean_object* x_195; 
+lean_dec(x_35);
+lean_dec(x_24);
+lean_dec(x_19);
+lean_dec(x_10);
+lean_dec(x_7);
+lean_dec(x_6);
+lean_dec(x_5);
+lean_dec(x_4);
+lean_dec(x_3);
+lean_dec(x_2);
+lean_dec(x_1);
+x_194 = lean_box(0);
+if (lean_is_scalar(x_12)) {
+ x_195 = lean_alloc_ctor(0, 2, 0);
+} else {
+ x_195 = x_12;
+}
+lean_ctor_set(x_195, 0, x_194);
+lean_ctor_set(x_195, 1, x_29);
+return x_195;
+}
+}
+}
+block_219:
+{
+if (x_197 == 0)
+{
+lean_dec(x_14);
+x_29 = x_198;
+goto block_196;
+}
+else
+{
+lean_object* x_199; lean_object* x_200; lean_object* x_201; lean_object* x_202; lean_object* x_203; lean_object* x_204; lean_object* x_205; lean_object* x_206; lean_object* x_207; lean_object* x_208; lean_object* x_209; lean_object* x_210; lean_object* x_211; lean_object* x_212; lean_object* x_213; lean_object* x_214; lean_object* x_215; lean_object* x_216; lean_object* x_217; lean_object* x_218; 
+x_199 = lean_array_get_size(x_14);
+lean_dec(x_14);
+x_200 = l_Lean_fmt___at_Lean_Position_instToFormatPosition___spec__1(x_199);
+x_201 = lean_alloc_ctor(0, 1, 0);
+lean_ctor_set(x_201, 0, x_200);
+x_202 = l___private_Lean_Elab_App_0__Lean_Elab_Term_ElabAppArgs_propagateExpectedType___closed__5;
+x_203 = lean_alloc_ctor(10, 2, 0);
+lean_ctor_set(x_203, 0, x_202);
+lean_ctor_set(x_203, 1, x_201);
+x_204 = l___private_Lean_Elab_App_0__Lean_Elab_Term_ElabAppArgs_propagateExpectedType___closed__7;
+x_205 = lean_alloc_ctor(10, 2, 0);
+lean_ctor_set(x_205, 0, x_203);
+lean_ctor_set(x_205, 1, x_204);
+lean_inc(x_28);
+x_206 = l_Lean_fmt___at_Lean_Position_instToFormatPosition___spec__1(x_28);
+x_207 = lean_alloc_ctor(0, 1, 0);
+lean_ctor_set(x_207, 0, x_206);
+x_208 = lean_alloc_ctor(10, 2, 0);
+lean_ctor_set(x_208, 0, x_205);
+lean_ctor_set(x_208, 1, x_207);
+x_209 = l___private_Lean_Elab_App_0__Lean_Elab_Term_ElabAppArgs_propagateExpectedType___closed__9;
+x_210 = lean_alloc_ctor(10, 2, 0);
+lean_ctor_set(x_210, 0, x_208);
+lean_ctor_set(x_210, 1, x_209);
+x_211 = lean_ctor_get(x_10, 1);
 lean_inc(x_211);
-lean_inc(x_210);
-lean_inc(x_209);
-lean_inc(x_207);
-lean_inc(x_206);
-lean_inc(x_205);
-lean_inc(x_204);
-lean_dec(x_21);
-x_214 = 1;
-x_215 = lean_alloc_ctor(0, 9, 3);
-lean_ctor_set(x_215, 0, x_204);
-lean_ctor_set(x_215, 1, x_205);
-lean_ctor_set(x_215, 2, x_206);
-lean_ctor_set(x_215, 3, x_207);
-lean_ctor_set(x_215, 4, x_209);
-lean_ctor_set(x_215, 5, x_210);
-lean_ctor_set(x_215, 6, x_211);
-lean_ctor_set(x_215, 7, x_212);
-lean_ctor_set(x_215, 8, x_213);
-lean_ctor_set_uint8(x_215, sizeof(void*)*9, x_203);
-lean_ctor_set_uint8(x_215, sizeof(void*)*9 + 1, x_208);
-lean_ctor_set_uint8(x_215, sizeof(void*)*9 + 2, x_214);
-x_216 = lean_st_ref_set(x_1, x_215, x_22);
-x_217 = lean_ctor_get(x_11, 4);
-lean_inc(x_217);
-if (lean_obj_tag(x_217) == 0)
-{
-lean_object* x_218; lean_object* x_219; lean_object* x_220; lean_object* x_221; 
-lean_dec(x_18);
-lean_dec(x_14);
-lean_dec(x_11);
-lean_dec(x_7);
-lean_dec(x_6);
-lean_dec(x_5);
-lean_dec(x_4);
-lean_dec(x_3);
-lean_dec(x_2);
-lean_dec(x_1);
-x_218 = lean_ctor_get(x_216, 1);
+x_212 = lean_alloc_ctor(2, 1, 0);
+lean_ctor_set(x_212, 0, x_211);
+x_213 = lean_alloc_ctor(10, 2, 0);
+lean_ctor_set(x_213, 0, x_210);
+lean_ctor_set(x_213, 1, x_212);
+x_214 = l_Array_foldlMUnsafe_fold___at_Lean_withNestedTraces___spec__5___closed__1;
+x_215 = lean_alloc_ctor(10, 2, 0);
+lean_ctor_set(x_215, 0, x_213);
+lean_ctor_set(x_215, 1, x_214);
+x_216 = l___private_Lean_Elab_App_0__Lean_Elab_Term_ElabAppArgs_propagateExpectedType___closed__3;
+x_217 = l_Lean_addTrace___at___private_Lean_Elab_App_0__Lean_Elab_Term_ElabAppArgs_propagateExpectedType___spec__6(x_216, x_215, x_1, x_2, x_3, x_4, x_5, x_6, x_7, x_198);
+x_218 = lean_ctor_get(x_217, 1);
 lean_inc(x_218);
-if (lean_is_exclusive(x_216)) {
- lean_ctor_release(x_216, 0);
- lean_ctor_release(x_216, 1);
- x_219 = x_216;
-} else {
- lean_dec_ref(x_216);
- x_219 = lean_box(0);
-}
-x_220 = lean_box(0);
-if (lean_is_scalar(x_219)) {
- x_221 = lean_alloc_ctor(0, 2, 0);
-} else {
- x_221 = x_219;
-}
-lean_ctor_set(x_221, 0, x_220);
-lean_ctor_set(x_221, 1, x_218);
-return x_221;
-}
-else
-{
-lean_object* x_222; lean_object* x_223; lean_object* x_224; uint8_t x_225; 
-x_222 = lean_ctor_get(x_216, 1);
-lean_inc(x_222);
-if (lean_is_exclusive(x_216)) {
- lean_ctor_release(x_216, 0);
- lean_ctor_release(x_216, 1);
- x_223 = x_216;
-} else {
- lean_dec_ref(x_216);
- x_223 = lean_box(0);
-}
-x_224 = lean_ctor_get(x_217, 0);
-lean_inc(x_224);
 lean_dec(x_217);
-x_225 = l_Lean_Expr_isProp(x_224);
-if (x_225 == 0)
-{
-lean_object* x_226; lean_object* x_227; lean_object* x_228; lean_object* x_229; uint8_t x_303; lean_object* x_304; lean_object* x_326; lean_object* x_327; lean_object* x_328; uint8_t x_329; 
-x_226 = lean_ctor_get(x_11, 2);
-lean_inc(x_226);
-x_227 = lean_unsigned_to_nat(0u);
-x_228 = l_List_lengthAux___rarg(x_226, x_227);
-lean_dec(x_226);
-x_326 = lean_st_ref_get(x_7, x_222);
-x_327 = lean_ctor_get(x_326, 0);
-lean_inc(x_327);
-x_328 = lean_ctor_get(x_327, 3);
-lean_inc(x_328);
-lean_dec(x_327);
-x_329 = lean_ctor_get_uint8(x_328, sizeof(void*)*1);
-lean_dec(x_328);
-if (x_329 == 0)
-{
-lean_object* x_330; uint8_t x_331; 
-x_330 = lean_ctor_get(x_326, 1);
-lean_inc(x_330);
-lean_dec(x_326);
-x_331 = 0;
-x_303 = x_331;
-x_304 = x_330;
-goto block_325;
+x_29 = x_218;
+goto block_196;
+}
+}
 }
 else
 {
-lean_object* x_332; lean_object* x_333; lean_object* x_334; lean_object* x_335; lean_object* x_336; uint8_t x_337; 
-x_332 = lean_ctor_get(x_326, 1);
-lean_inc(x_332);
-lean_dec(x_326);
-x_333 = l___private_Lean_Elab_App_0__Lean_Elab_Term_ElabAppArgs_propagateExpectedType___closed__3;
-x_334 = l___private_Lean_Util_Trace_0__Lean_checkTraceOptionM___at___private_Lean_Elab_App_0__Lean_Elab_Term_ElabAppArgs_propagateExpectedType___spec__7(x_333, x_1, x_2, x_3, x_4, x_5, x_6, x_7, x_332);
-x_335 = lean_ctor_get(x_334, 0);
-lean_inc(x_335);
-x_336 = lean_ctor_get(x_334, 1);
-lean_inc(x_336);
-lean_dec(x_334);
-x_337 = lean_unbox(x_335);
-lean_dec(x_335);
-x_303 = x_337;
-x_304 = x_336;
-goto block_325;
-}
-block_302:
-{
-lean_object* x_230; lean_object* x_231; lean_object* x_232; 
-x_230 = lean_ctor_get(x_11, 3);
-lean_inc(x_230);
-x_231 = lean_ctor_get(x_11, 1);
-lean_inc(x_231);
-x_232 = l___private_Lean_Elab_App_0__Lean_Elab_Term_ElabAppArgs_getForallBody(x_228, x_230, x_231);
-if (lean_obj_tag(x_232) == 0)
-{
-lean_object* x_233; lean_object* x_234; 
-lean_dec(x_224);
-lean_dec(x_18);
-lean_dec(x_11);
+lean_object* x_232; lean_object* x_233; lean_object* x_234; uint8_t x_235; 
+lean_dec(x_24);
+lean_dec(x_19);
+lean_dec(x_14);
+lean_dec(x_12);
+lean_dec(x_10);
 lean_dec(x_7);
 lean_dec(x_6);
 lean_dec(x_5);
 lean_dec(x_4);
 lean_dec(x_3);
 lean_dec(x_2);
-lean_dec(x_1);
-x_233 = lean_box(0);
-if (lean_is_scalar(x_223)) {
- x_234 = lean_alloc_ctor(0, 2, 0);
-} else {
- x_234 = x_223;
-}
-lean_ctor_set(x_234, 0, x_233);
-lean_ctor_set(x_234, 1, x_229);
-return x_234;
-}
-else
-{
-lean_object* x_235; uint8_t x_236; 
-x_235 = lean_ctor_get(x_232, 0);
-lean_inc(x_235);
+x_232 = lean_st_ref_take(x_1, x_11);
+x_233 = lean_ctor_get(x_232, 0);
+lean_inc(x_233);
+x_234 = lean_ctor_get(x_232, 1);
+lean_inc(x_234);
 lean_dec(x_232);
-x_236 = l_Lean_Expr_hasLooseBVars(x_235);
-if (x_236 == 0)
+x_235 = !lean_is_exclusive(x_233);
+if (x_235 == 0)
 {
-lean_object* x_237; lean_object* x_238; 
-x_237 = lean_box(0);
-lean_inc(x_235);
-x_238 = l_Lean_FindMVar_main___at___private_Lean_Elab_App_0__Lean_Elab_Term_ElabAppArgs_propagateExpectedType___spec__1(x_11, x_235, x_237);
-if (lean_obj_tag(x_238) == 0)
+uint8_t x_236; lean_object* x_237; uint8_t x_238; 
+x_236 = 1;
+lean_ctor_set_uint8(x_233, sizeof(void*)*9 + 2, x_236);
+x_237 = lean_st_ref_set(x_1, x_233, x_234);
+lean_dec(x_1);
+x_238 = !lean_is_exclusive(x_237);
+if (x_238 == 0)
 {
 lean_object* x_239; lean_object* x_240; 
-lean_dec(x_235);
-lean_dec(x_224);
-lean_dec(x_18);
-lean_dec(x_7);
-lean_dec(x_6);
-lean_dec(x_5);
-lean_dec(x_4);
-lean_dec(x_3);
-lean_dec(x_2);
-lean_dec(x_1);
-x_239 = lean_box(0);
-if (lean_is_scalar(x_223)) {
- x_240 = lean_alloc_ctor(0, 2, 0);
-} else {
- x_240 = x_223;
-}
-lean_ctor_set(x_240, 0, x_239);
-lean_ctor_set(x_240, 1, x_229);
-return x_240;
+x_239 = lean_ctor_get(x_237, 0);
+lean_dec(x_239);
+x_240 = lean_box(0);
+lean_ctor_set(x_237, 0, x_240);
+return x_237;
 }
 else
 {
-lean_object* x_241; 
-lean_dec(x_238);
-lean_inc(x_235);
-x_241 = l_Lean_FindMVar_main___at___private_Lean_Elab_App_0__Lean_Elab_Term_ElabAppArgs_propagateExpectedType___spec__2(x_18, x_235, x_237);
-if (lean_obj_tag(x_241) == 0)
-{
-lean_object* x_242; lean_object* x_243; 
-lean_dec(x_223);
-x_242 = l___private_Lean_Elab_App_0__Lean_Elab_Term_ElabAppArgs_hasOptAutoParams___closed__1;
-lean_inc(x_7);
-lean_inc(x_6);
-lean_inc(x_5);
-lean_inc(x_4);
-lean_inc(x_3);
-lean_inc(x_2);
-lean_inc(x_1);
-lean_inc(x_235);
-x_243 = l_Lean_Meta_forallTelescopeReducing___at___private_Lean_Elab_App_0__Lean_Elab_Term_ElabAppArgs_hasOptAutoParams___spec__2___rarg(x_235, x_242, x_1, x_2, x_3, x_4, x_5, x_6, x_7, x_229);
-if (lean_obj_tag(x_243) == 0)
-{
-lean_object* x_244; lean_object* x_245; lean_object* x_246; uint8_t x_247; lean_object* x_248; uint8_t x_279; 
-x_244 = lean_ctor_get(x_243, 0);
-lean_inc(x_244);
-x_245 = lean_ctor_get(x_243, 1);
-lean_inc(x_245);
-if (lean_is_exclusive(x_243)) {
- lean_ctor_release(x_243, 0);
- lean_ctor_release(x_243, 1);
- x_246 = x_243;
-} else {
- lean_dec_ref(x_243);
- x_246 = lean_box(0);
-}
-x_279 = lean_unbox(x_244);
-lean_dec(x_244);
-if (x_279 == 0)
-{
-lean_object* x_280; lean_object* x_281; lean_object* x_282; uint8_t x_283; 
-lean_dec(x_246);
-x_280 = lean_st_ref_get(x_7, x_245);
-x_281 = lean_ctor_get(x_280, 0);
-lean_inc(x_281);
-x_282 = lean_ctor_get(x_281, 3);
-lean_inc(x_282);
-lean_dec(x_281);
-x_283 = lean_ctor_get_uint8(x_282, sizeof(void*)*1);
-lean_dec(x_282);
-if (x_283 == 0)
-{
-lean_object* x_284; uint8_t x_285; 
-x_284 = lean_ctor_get(x_280, 1);
-lean_inc(x_284);
-lean_dec(x_280);
-x_285 = 0;
-x_247 = x_285;
-x_248 = x_284;
-goto block_278;
-}
-else
-{
-lean_object* x_286; lean_object* x_287; lean_object* x_288; lean_object* x_289; lean_object* x_290; uint8_t x_291; 
-x_286 = lean_ctor_get(x_280, 1);
-lean_inc(x_286);
-lean_dec(x_280);
-x_287 = l___private_Lean_Elab_App_0__Lean_Elab_Term_ElabAppArgs_propagateExpectedType___closed__3;
-x_288 = l___private_Lean_Util_Trace_0__Lean_checkTraceOptionM___at___private_Lean_Elab_App_0__Lean_Elab_Term_ElabAppArgs_propagateExpectedType___spec__7(x_287, x_1, x_2, x_3, x_4, x_5, x_6, x_7, x_286);
-x_289 = lean_ctor_get(x_288, 0);
-lean_inc(x_289);
-x_290 = lean_ctor_get(x_288, 1);
-lean_inc(x_290);
-lean_dec(x_288);
-x_291 = lean_unbox(x_289);
-lean_dec(x_289);
-x_247 = x_291;
-x_248 = x_290;
-goto block_278;
+lean_object* x_241; lean_object* x_242; lean_object* x_243; 
+x_241 = lean_ctor_get(x_237, 1);
+lean_inc(x_241);
+lean_dec(x_237);
+x_242 = lean_box(0);
+x_243 = lean_alloc_ctor(0, 2, 0);
+lean_ctor_set(x_243, 0, x_242);
+lean_ctor_set(x_243, 1, x_241);
+return x_243;
 }
 }
 else
 {
-lean_object* x_292; lean_object* x_293; 
-lean_dec(x_235);
-lean_dec(x_224);
-lean_dec(x_7);
-lean_dec(x_6);
-lean_dec(x_5);
-lean_dec(x_4);
-lean_dec(x_3);
-lean_dec(x_2);
-lean_dec(x_1);
-x_292 = lean_box(0);
-if (lean_is_scalar(x_246)) {
- x_293 = lean_alloc_ctor(0, 2, 0);
-} else {
- x_293 = x_246;
-}
-lean_ctor_set(x_293, 0, x_292);
-lean_ctor_set(x_293, 1, x_245);
-return x_293;
-}
-block_278:
-{
-if (x_247 == 0)
-{
-lean_object* x_249; 
-x_249 = l_Lean_Meta_isExprDefEq___at___private_Lean_Elab_App_0__Lean_Elab_Term_ElabAppArgs_propagateExpectedType___spec__3(x_224, x_235, x_1, x_2, x_3, x_4, x_5, x_6, x_7, x_248);
-lean_dec(x_3);
-lean_dec(x_2);
-lean_dec(x_1);
-if (lean_obj_tag(x_249) == 0)
-{
-lean_object* x_250; lean_object* x_251; lean_object* x_252; lean_object* x_253; 
-x_250 = lean_ctor_get(x_249, 1);
-lean_inc(x_250);
-if (lean_is_exclusive(x_249)) {
- lean_ctor_release(x_249, 0);
- lean_ctor_release(x_249, 1);
- x_251 = x_249;
-} else {
- lean_dec_ref(x_249);
- x_251 = lean_box(0);
-}
-x_252 = lean_box(0);
-if (lean_is_scalar(x_251)) {
- x_253 = lean_alloc_ctor(0, 2, 0);
-} else {
- x_253 = x_251;
-}
-lean_ctor_set(x_253, 0, x_252);
-lean_ctor_set(x_253, 1, x_250);
-return x_253;
-}
-else
-{
-lean_object* x_254; lean_object* x_255; lean_object* x_256; lean_object* x_257; 
-x_254 = lean_ctor_get(x_249, 0);
+uint8_t x_244; lean_object* x_245; lean_object* x_246; lean_object* x_247; lean_object* x_248; uint8_t x_249; lean_object* x_250; lean_object* x_251; lean_object* x_252; lean_object* x_253; lean_object* x_254; uint8_t x_255; lean_object* x_256; lean_object* x_257; lean_object* x_258; lean_object* x_259; lean_object* x_260; lean_object* x_261; 
+x_244 = lean_ctor_get_uint8(x_233, sizeof(void*)*9);
+x_245 = lean_ctor_get(x_233, 0);
+x_246 = lean_ctor_get(x_233, 1);
+x_247 = lean_ctor_get(x_233, 2);
+x_248 = lean_ctor_get(x_233, 3);
+x_249 = lean_ctor_get_uint8(x_233, sizeof(void*)*9 + 1);
+x_250 = lean_ctor_get(x_233, 4);
+x_251 = lean_ctor_get(x_233, 5);
+x_252 = lean_ctor_get(x_233, 6);
+x_253 = lean_ctor_get(x_233, 7);
+x_254 = lean_ctor_get(x_233, 8);
 lean_inc(x_254);
-x_255 = lean_ctor_get(x_249, 1);
-lean_inc(x_255);
-if (lean_is_exclusive(x_249)) {
- lean_ctor_release(x_249, 0);
- lean_ctor_release(x_249, 1);
- x_256 = x_249;
+lean_inc(x_253);
+lean_inc(x_252);
+lean_inc(x_251);
+lean_inc(x_250);
+lean_inc(x_248);
+lean_inc(x_247);
+lean_inc(x_246);
+lean_inc(x_245);
+lean_dec(x_233);
+x_255 = 1;
+x_256 = lean_alloc_ctor(0, 9, 3);
+lean_ctor_set(x_256, 0, x_245);
+lean_ctor_set(x_256, 1, x_246);
+lean_ctor_set(x_256, 2, x_247);
+lean_ctor_set(x_256, 3, x_248);
+lean_ctor_set(x_256, 4, x_250);
+lean_ctor_set(x_256, 5, x_251);
+lean_ctor_set(x_256, 6, x_252);
+lean_ctor_set(x_256, 7, x_253);
+lean_ctor_set(x_256, 8, x_254);
+lean_ctor_set_uint8(x_256, sizeof(void*)*9, x_244);
+lean_ctor_set_uint8(x_256, sizeof(void*)*9 + 1, x_249);
+lean_ctor_set_uint8(x_256, sizeof(void*)*9 + 2, x_255);
+x_257 = lean_st_ref_set(x_1, x_256, x_234);
+lean_dec(x_1);
+x_258 = lean_ctor_get(x_257, 1);
+lean_inc(x_258);
+if (lean_is_exclusive(x_257)) {
+ lean_ctor_release(x_257, 0);
+ lean_ctor_release(x_257, 1);
+ x_259 = x_257;
 } else {
- lean_dec_ref(x_249);
- x_256 = lean_box(0);
+ lean_dec_ref(x_257);
+ x_259 = lean_box(0);
 }
-if (lean_is_scalar(x_256)) {
- x_257 = lean_alloc_ctor(1, 2, 0);
+x_260 = lean_box(0);
+if (lean_is_scalar(x_259)) {
+ x_261 = lean_alloc_ctor(0, 2, 0);
 } else {
- x_257 = x_256;
+ x_261 = x_259;
 }
-lean_ctor_set(x_257, 0, x_254);
-lean_ctor_set(x_257, 1, x_255);
-return x_257;
+lean_ctor_set(x_261, 0, x_260);
+lean_ctor_set(x_261, 1, x_258);
+return x_261;
+}
+}
 }
 }
 else
 {
-lean_object* x_258; lean_object* x_259; lean_object* x_260; lean_object* x_261; lean_object* x_262; lean_object* x_263; lean_object* x_264; lean_object* x_265; lean_object* x_266; lean_object* x_267; lean_object* x_268; lean_object* x_269; 
-lean_inc(x_224);
-x_258 = lean_alloc_ctor(2, 1, 0);
-lean_ctor_set(x_258, 0, x_224);
-x_259 = l_Array_foldlMUnsafe_fold___at_Lean_withNestedTraces___spec__5___closed__1;
-x_260 = lean_alloc_ctor(10, 2, 0);
-lean_ctor_set(x_260, 0, x_259);
-lean_ctor_set(x_260, 1, x_258);
-x_261 = l_Lean_Meta_isLevelDefEqAux___closed__6;
-x_262 = lean_alloc_ctor(10, 2, 0);
-lean_ctor_set(x_262, 0, x_260);
-lean_ctor_set(x_262, 1, x_261);
-lean_inc(x_235);
-x_263 = lean_alloc_ctor(2, 1, 0);
-lean_ctor_set(x_263, 0, x_235);
-x_264 = lean_alloc_ctor(10, 2, 0);
-lean_ctor_set(x_264, 0, x_262);
-lean_ctor_set(x_264, 1, x_263);
-x_265 = lean_alloc_ctor(10, 2, 0);
+lean_object* x_262; lean_object* x_263; 
+lean_dec(x_19);
+lean_dec(x_14);
+lean_dec(x_10);
+lean_dec(x_7);
+lean_dec(x_6);
+lean_dec(x_5);
+lean_dec(x_4);
+lean_dec(x_3);
+lean_dec(x_2);
+lean_dec(x_1);
+x_262 = lean_box(0);
+if (lean_is_scalar(x_12)) {
+ x_263 = lean_alloc_ctor(0, 2, 0);
+} else {
+ x_263 = x_12;
+}
+lean_ctor_set(x_263, 0, x_262);
+lean_ctor_set(x_263, 1, x_11);
+return x_263;
+}
+}
+else
+{
+lean_object* x_264; lean_object* x_265; 
+lean_dec(x_14);
+lean_dec(x_10);
+lean_dec(x_7);
+lean_dec(x_6);
+lean_dec(x_5);
+lean_dec(x_4);
+lean_dec(x_3);
+lean_dec(x_2);
+lean_dec(x_1);
+x_264 = lean_box(0);
+if (lean_is_scalar(x_12)) {
+ x_265 = lean_alloc_ctor(0, 2, 0);
+} else {
+ x_265 = x_12;
+}
 lean_ctor_set(x_265, 0, x_264);
-lean_ctor_set(x_265, 1, x_259);
-x_266 = l___private_Lean_Elab_App_0__Lean_Elab_Term_ElabAppArgs_propagateExpectedType___closed__3;
-x_267 = l_Lean_addTrace___at___private_Lean_Elab_App_0__Lean_Elab_Term_ElabAppArgs_propagateExpectedType___spec__6(x_266, x_265, x_1, x_2, x_3, x_4, x_5, x_6, x_7, x_248);
-x_268 = lean_ctor_get(x_267, 1);
-lean_inc(x_268);
-lean_dec(x_267);
-x_269 = l_Lean_Meta_isExprDefEq___at___private_Lean_Elab_App_0__Lean_Elab_Term_ElabAppArgs_propagateExpectedType___spec__3(x_224, x_235, x_1, x_2, x_3, x_4, x_5, x_6, x_7, x_268);
-lean_dec(x_3);
-lean_dec(x_2);
-lean_dec(x_1);
-if (lean_obj_tag(x_269) == 0)
-{
-lean_object* x_270; lean_object* x_271; lean_object* x_272; lean_object* x_273; 
-x_270 = lean_ctor_get(x_269, 1);
-lean_inc(x_270);
-if (lean_is_exclusive(x_269)) {
- lean_ctor_release(x_269, 0);
- lean_ctor_release(x_269, 1);
- x_271 = x_269;
-} else {
- lean_dec_ref(x_269);
- x_271 = lean_box(0);
-}
-x_272 = lean_box(0);
-if (lean_is_scalar(x_271)) {
- x_273 = lean_alloc_ctor(0, 2, 0);
-} else {
- x_273 = x_271;
-}
-lean_ctor_set(x_273, 0, x_272);
-lean_ctor_set(x_273, 1, x_270);
-return x_273;
-}
-else
-{
-lean_object* x_274; lean_object* x_275; lean_object* x_276; lean_object* x_277; 
-x_274 = lean_ctor_get(x_269, 0);
-lean_inc(x_274);
-x_275 = lean_ctor_get(x_269, 1);
-lean_inc(x_275);
-if (lean_is_exclusive(x_269)) {
- lean_ctor_release(x_269, 0);
- lean_ctor_release(x_269, 1);
- x_276 = x_269;
-} else {
- lean_dec_ref(x_269);
- x_276 = lean_box(0);
-}
-if (lean_is_scalar(x_276)) {
- x_277 = lean_alloc_ctor(1, 2, 0);
-} else {
- x_277 = x_276;
-}
-lean_ctor_set(x_277, 0, x_274);
-lean_ctor_set(x_277, 1, x_275);
-return x_277;
-}
-}
+lean_ctor_set(x_265, 1, x_11);
+return x_265;
 }
 }
 else
 {
-lean_object* x_294; lean_object* x_295; lean_object* x_296; lean_object* x_297; 
-lean_dec(x_235);
-lean_dec(x_224);
-lean_dec(x_7);
-lean_dec(x_6);
-lean_dec(x_5);
-lean_dec(x_4);
-lean_dec(x_3);
-lean_dec(x_2);
-lean_dec(x_1);
-x_294 = lean_ctor_get(x_243, 0);
-lean_inc(x_294);
-x_295 = lean_ctor_get(x_243, 1);
-lean_inc(x_295);
-if (lean_is_exclusive(x_243)) {
- lean_ctor_release(x_243, 0);
- lean_ctor_release(x_243, 1);
- x_296 = x_243;
-} else {
- lean_dec_ref(x_243);
- x_296 = lean_box(0);
-}
-if (lean_is_scalar(x_296)) {
- x_297 = lean_alloc_ctor(1, 2, 0);
-} else {
- x_297 = x_296;
-}
-lean_ctor_set(x_297, 0, x_294);
-lean_ctor_set(x_297, 1, x_295);
-return x_297;
-}
-}
-else
-{
-lean_object* x_298; lean_object* x_299; 
-lean_dec(x_241);
-lean_dec(x_235);
-lean_dec(x_224);
-lean_dec(x_7);
-lean_dec(x_6);
-lean_dec(x_5);
-lean_dec(x_4);
-lean_dec(x_3);
-lean_dec(x_2);
-lean_dec(x_1);
-x_298 = lean_box(0);
-if (lean_is_scalar(x_223)) {
- x_299 = lean_alloc_ctor(0, 2, 0);
-} else {
- x_299 = x_223;
-}
-lean_ctor_set(x_299, 0, x_298);
-lean_ctor_set(x_299, 1, x_229);
-return x_299;
-}
-}
-}
-else
-{
-lean_object* x_300; lean_object* x_301; 
-lean_dec(x_235);
-lean_dec(x_224);
-lean_dec(x_18);
-lean_dec(x_11);
-lean_dec(x_7);
-lean_dec(x_6);
-lean_dec(x_5);
-lean_dec(x_4);
-lean_dec(x_3);
-lean_dec(x_2);
-lean_dec(x_1);
-x_300 = lean_box(0);
-if (lean_is_scalar(x_223)) {
- x_301 = lean_alloc_ctor(0, 2, 0);
-} else {
- x_301 = x_223;
-}
-lean_ctor_set(x_301, 0, x_300);
-lean_ctor_set(x_301, 1, x_229);
-return x_301;
-}
-}
-}
-block_325:
-{
-if (x_303 == 0)
-{
+lean_object* x_266; lean_object* x_267; 
 lean_dec(x_14);
-x_229 = x_304;
-goto block_302;
-}
-else
-{
-lean_object* x_305; lean_object* x_306; lean_object* x_307; lean_object* x_308; lean_object* x_309; lean_object* x_310; lean_object* x_311; lean_object* x_312; lean_object* x_313; lean_object* x_314; lean_object* x_315; lean_object* x_316; lean_object* x_317; lean_object* x_318; lean_object* x_319; lean_object* x_320; lean_object* x_321; lean_object* x_322; lean_object* x_323; lean_object* x_324; 
-x_305 = lean_array_get_size(x_14);
-lean_dec(x_14);
-x_306 = l_Lean_fmt___at_Lean_Position_instToFormatPosition___spec__1(x_305);
-x_307 = lean_alloc_ctor(0, 1, 0);
-lean_ctor_set(x_307, 0, x_306);
-x_308 = l___private_Lean_Elab_App_0__Lean_Elab_Term_ElabAppArgs_propagateExpectedType___closed__5;
-x_309 = lean_alloc_ctor(10, 2, 0);
-lean_ctor_set(x_309, 0, x_308);
-lean_ctor_set(x_309, 1, x_307);
-x_310 = l___private_Lean_Elab_App_0__Lean_Elab_Term_ElabAppArgs_propagateExpectedType___closed__7;
-x_311 = lean_alloc_ctor(10, 2, 0);
-lean_ctor_set(x_311, 0, x_309);
-lean_ctor_set(x_311, 1, x_310);
-lean_inc(x_228);
-x_312 = l_Lean_fmt___at_Lean_Position_instToFormatPosition___spec__1(x_228);
-x_313 = lean_alloc_ctor(0, 1, 0);
-lean_ctor_set(x_313, 0, x_312);
-x_314 = lean_alloc_ctor(10, 2, 0);
-lean_ctor_set(x_314, 0, x_311);
-lean_ctor_set(x_314, 1, x_313);
-x_315 = l___private_Lean_Elab_App_0__Lean_Elab_Term_ElabAppArgs_propagateExpectedType___closed__9;
-x_316 = lean_alloc_ctor(10, 2, 0);
-lean_ctor_set(x_316, 0, x_314);
-lean_ctor_set(x_316, 1, x_315);
-x_317 = lean_ctor_get(x_11, 1);
-lean_inc(x_317);
-x_318 = lean_alloc_ctor(2, 1, 0);
-lean_ctor_set(x_318, 0, x_317);
-x_319 = lean_alloc_ctor(10, 2, 0);
-lean_ctor_set(x_319, 0, x_316);
-lean_ctor_set(x_319, 1, x_318);
-x_320 = l_Array_foldlMUnsafe_fold___at_Lean_withNestedTraces___spec__5___closed__1;
-x_321 = lean_alloc_ctor(10, 2, 0);
-lean_ctor_set(x_321, 0, x_319);
-lean_ctor_set(x_321, 1, x_320);
-x_322 = l___private_Lean_Elab_App_0__Lean_Elab_Term_ElabAppArgs_propagateExpectedType___closed__3;
-x_323 = l_Lean_addTrace___at___private_Lean_Elab_App_0__Lean_Elab_Term_ElabAppArgs_propagateExpectedType___spec__6(x_322, x_321, x_1, x_2, x_3, x_4, x_5, x_6, x_7, x_304);
-x_324 = lean_ctor_get(x_323, 1);
-lean_inc(x_324);
-lean_dec(x_323);
-x_229 = x_324;
-goto block_302;
-}
-}
-}
-else
-{
-lean_object* x_338; lean_object* x_339; 
-lean_dec(x_224);
-lean_dec(x_18);
-lean_dec(x_14);
-lean_dec(x_11);
+lean_dec(x_10);
 lean_dec(x_7);
 lean_dec(x_6);
 lean_dec(x_5);
@@ -14746,807 +14388,15 @@ lean_dec(x_4);
 lean_dec(x_3);
 lean_dec(x_2);
 lean_dec(x_1);
-x_338 = lean_box(0);
-if (lean_is_scalar(x_223)) {
- x_339 = lean_alloc_ctor(0, 2, 0);
+x_266 = lean_box(0);
+if (lean_is_scalar(x_12)) {
+ x_267 = lean_alloc_ctor(0, 2, 0);
 } else {
- x_339 = x_223;
-}
-lean_ctor_set(x_339, 0, x_338);
-lean_ctor_set(x_339, 1, x_222);
-return x_339;
-}
-}
-}
-}
-else
-{
-lean_object* x_340; 
-lean_dec(x_18);
-lean_dec(x_14);
-lean_dec(x_11);
-lean_dec(x_7);
-lean_dec(x_6);
-lean_dec(x_5);
-lean_dec(x_4);
-lean_dec(x_3);
-lean_dec(x_2);
-lean_dec(x_1);
-x_340 = lean_box(0);
-lean_ctor_set(x_9, 0, x_340);
-return x_9;
-}
-}
-else
-{
-lean_object* x_341; 
-lean_dec(x_14);
-lean_dec(x_11);
-lean_dec(x_7);
-lean_dec(x_6);
-lean_dec(x_5);
-lean_dec(x_4);
-lean_dec(x_3);
-lean_dec(x_2);
-lean_dec(x_1);
-x_341 = lean_box(0);
-lean_ctor_set(x_9, 0, x_341);
-return x_9;
-}
-}
-else
-{
-lean_object* x_342; 
-lean_dec(x_14);
-lean_dec(x_11);
-lean_dec(x_7);
-lean_dec(x_6);
-lean_dec(x_5);
-lean_dec(x_4);
-lean_dec(x_3);
-lean_dec(x_2);
-lean_dec(x_1);
-x_342 = lean_box(0);
-lean_ctor_set(x_9, 0, x_342);
-return x_9;
-}
-}
-}
-else
-{
-lean_object* x_343; lean_object* x_344; uint8_t x_345; lean_object* x_346; uint8_t x_347; 
-x_343 = lean_ctor_get(x_9, 0);
-x_344 = lean_ctor_get(x_9, 1);
-lean_inc(x_344);
-lean_inc(x_343);
-lean_dec(x_9);
-x_345 = lean_ctor_get_uint8(x_343, sizeof(void*)*9);
-x_346 = lean_ctor_get(x_343, 5);
-lean_inc(x_346);
-x_347 = l_Array_isEmpty___rarg(x_346);
-if (x_347 == 0)
-{
-lean_object* x_348; lean_object* x_349; 
-lean_dec(x_346);
-lean_dec(x_343);
-lean_dec(x_7);
-lean_dec(x_6);
-lean_dec(x_5);
-lean_dec(x_4);
-lean_dec(x_3);
-lean_dec(x_2);
-lean_dec(x_1);
-x_348 = lean_box(0);
-x_349 = lean_alloc_ctor(0, 2, 0);
-lean_ctor_set(x_349, 0, x_348);
-lean_ctor_set(x_349, 1, x_344);
-return x_349;
-}
-else
-{
-if (x_345 == 0)
-{
-uint8_t x_350; 
-x_350 = lean_ctor_get_uint8(x_343, sizeof(void*)*9 + 2);
-if (x_350 == 0)
-{
-lean_object* x_351; uint8_t x_352; 
-x_351 = lean_ctor_get(x_343, 8);
-lean_inc(x_351);
-x_352 = l_Array_isEmpty___rarg(x_351);
-if (x_352 == 0)
-{
-lean_object* x_353; lean_object* x_354; lean_object* x_355; uint8_t x_356; lean_object* x_357; lean_object* x_358; lean_object* x_359; lean_object* x_360; uint8_t x_361; lean_object* x_362; lean_object* x_363; lean_object* x_364; lean_object* x_365; lean_object* x_366; lean_object* x_367; uint8_t x_368; lean_object* x_369; lean_object* x_370; lean_object* x_371; 
-x_353 = lean_st_ref_take(x_1, x_344);
-x_354 = lean_ctor_get(x_353, 0);
-lean_inc(x_354);
-x_355 = lean_ctor_get(x_353, 1);
-lean_inc(x_355);
-lean_dec(x_353);
-x_356 = lean_ctor_get_uint8(x_354, sizeof(void*)*9);
-x_357 = lean_ctor_get(x_354, 0);
-lean_inc(x_357);
-x_358 = lean_ctor_get(x_354, 1);
-lean_inc(x_358);
-x_359 = lean_ctor_get(x_354, 2);
-lean_inc(x_359);
-x_360 = lean_ctor_get(x_354, 3);
-lean_inc(x_360);
-x_361 = lean_ctor_get_uint8(x_354, sizeof(void*)*9 + 1);
-x_362 = lean_ctor_get(x_354, 4);
-lean_inc(x_362);
-x_363 = lean_ctor_get(x_354, 5);
-lean_inc(x_363);
-x_364 = lean_ctor_get(x_354, 6);
-lean_inc(x_364);
-x_365 = lean_ctor_get(x_354, 7);
-lean_inc(x_365);
-x_366 = lean_ctor_get(x_354, 8);
-lean_inc(x_366);
-if (lean_is_exclusive(x_354)) {
- lean_ctor_release(x_354, 0);
- lean_ctor_release(x_354, 1);
- lean_ctor_release(x_354, 2);
- lean_ctor_release(x_354, 3);
- lean_ctor_release(x_354, 4);
- lean_ctor_release(x_354, 5);
- lean_ctor_release(x_354, 6);
- lean_ctor_release(x_354, 7);
- lean_ctor_release(x_354, 8);
- x_367 = x_354;
-} else {
- lean_dec_ref(x_354);
- x_367 = lean_box(0);
-}
-x_368 = 1;
-if (lean_is_scalar(x_367)) {
- x_369 = lean_alloc_ctor(0, 9, 3);
-} else {
- x_369 = x_367;
-}
-lean_ctor_set(x_369, 0, x_357);
-lean_ctor_set(x_369, 1, x_358);
-lean_ctor_set(x_369, 2, x_359);
-lean_ctor_set(x_369, 3, x_360);
-lean_ctor_set(x_369, 4, x_362);
-lean_ctor_set(x_369, 5, x_363);
-lean_ctor_set(x_369, 6, x_364);
-lean_ctor_set(x_369, 7, x_365);
-lean_ctor_set(x_369, 8, x_366);
-lean_ctor_set_uint8(x_369, sizeof(void*)*9, x_356);
-lean_ctor_set_uint8(x_369, sizeof(void*)*9 + 1, x_361);
-lean_ctor_set_uint8(x_369, sizeof(void*)*9 + 2, x_368);
-x_370 = lean_st_ref_set(x_1, x_369, x_355);
-x_371 = lean_ctor_get(x_343, 4);
-lean_inc(x_371);
-if (lean_obj_tag(x_371) == 0)
-{
-lean_object* x_372; lean_object* x_373; lean_object* x_374; lean_object* x_375; 
-lean_dec(x_351);
-lean_dec(x_346);
-lean_dec(x_343);
-lean_dec(x_7);
-lean_dec(x_6);
-lean_dec(x_5);
-lean_dec(x_4);
-lean_dec(x_3);
-lean_dec(x_2);
-lean_dec(x_1);
-x_372 = lean_ctor_get(x_370, 1);
-lean_inc(x_372);
-if (lean_is_exclusive(x_370)) {
- lean_ctor_release(x_370, 0);
- lean_ctor_release(x_370, 1);
- x_373 = x_370;
-} else {
- lean_dec_ref(x_370);
- x_373 = lean_box(0);
-}
-x_374 = lean_box(0);
-if (lean_is_scalar(x_373)) {
- x_375 = lean_alloc_ctor(0, 2, 0);
-} else {
- x_375 = x_373;
-}
-lean_ctor_set(x_375, 0, x_374);
-lean_ctor_set(x_375, 1, x_372);
-return x_375;
-}
-else
-{
-lean_object* x_376; lean_object* x_377; lean_object* x_378; uint8_t x_379; 
-x_376 = lean_ctor_get(x_370, 1);
-lean_inc(x_376);
-if (lean_is_exclusive(x_370)) {
- lean_ctor_release(x_370, 0);
- lean_ctor_release(x_370, 1);
- x_377 = x_370;
-} else {
- lean_dec_ref(x_370);
- x_377 = lean_box(0);
-}
-x_378 = lean_ctor_get(x_371, 0);
-lean_inc(x_378);
-lean_dec(x_371);
-x_379 = l_Lean_Expr_isProp(x_378);
-if (x_379 == 0)
-{
-lean_object* x_380; lean_object* x_381; lean_object* x_382; lean_object* x_383; uint8_t x_457; lean_object* x_458; lean_object* x_480; lean_object* x_481; lean_object* x_482; uint8_t x_483; 
-x_380 = lean_ctor_get(x_343, 2);
-lean_inc(x_380);
-x_381 = lean_unsigned_to_nat(0u);
-x_382 = l_List_lengthAux___rarg(x_380, x_381);
-lean_dec(x_380);
-x_480 = lean_st_ref_get(x_7, x_376);
-x_481 = lean_ctor_get(x_480, 0);
-lean_inc(x_481);
-x_482 = lean_ctor_get(x_481, 3);
-lean_inc(x_482);
-lean_dec(x_481);
-x_483 = lean_ctor_get_uint8(x_482, sizeof(void*)*1);
-lean_dec(x_482);
-if (x_483 == 0)
-{
-lean_object* x_484; uint8_t x_485; 
-x_484 = lean_ctor_get(x_480, 1);
-lean_inc(x_484);
-lean_dec(x_480);
-x_485 = 0;
-x_457 = x_485;
-x_458 = x_484;
-goto block_479;
-}
-else
-{
-lean_object* x_486; lean_object* x_487; lean_object* x_488; lean_object* x_489; lean_object* x_490; uint8_t x_491; 
-x_486 = lean_ctor_get(x_480, 1);
-lean_inc(x_486);
-lean_dec(x_480);
-x_487 = l___private_Lean_Elab_App_0__Lean_Elab_Term_ElabAppArgs_propagateExpectedType___closed__3;
-x_488 = l___private_Lean_Util_Trace_0__Lean_checkTraceOptionM___at___private_Lean_Elab_App_0__Lean_Elab_Term_ElabAppArgs_propagateExpectedType___spec__7(x_487, x_1, x_2, x_3, x_4, x_5, x_6, x_7, x_486);
-x_489 = lean_ctor_get(x_488, 0);
-lean_inc(x_489);
-x_490 = lean_ctor_get(x_488, 1);
-lean_inc(x_490);
-lean_dec(x_488);
-x_491 = lean_unbox(x_489);
-lean_dec(x_489);
-x_457 = x_491;
-x_458 = x_490;
-goto block_479;
-}
-block_456:
-{
-lean_object* x_384; lean_object* x_385; lean_object* x_386; 
-x_384 = lean_ctor_get(x_343, 3);
-lean_inc(x_384);
-x_385 = lean_ctor_get(x_343, 1);
-lean_inc(x_385);
-x_386 = l___private_Lean_Elab_App_0__Lean_Elab_Term_ElabAppArgs_getForallBody(x_382, x_384, x_385);
-if (lean_obj_tag(x_386) == 0)
-{
-lean_object* x_387; lean_object* x_388; 
-lean_dec(x_378);
-lean_dec(x_351);
-lean_dec(x_343);
-lean_dec(x_7);
-lean_dec(x_6);
-lean_dec(x_5);
-lean_dec(x_4);
-lean_dec(x_3);
-lean_dec(x_2);
-lean_dec(x_1);
-x_387 = lean_box(0);
-if (lean_is_scalar(x_377)) {
- x_388 = lean_alloc_ctor(0, 2, 0);
-} else {
- x_388 = x_377;
-}
-lean_ctor_set(x_388, 0, x_387);
-lean_ctor_set(x_388, 1, x_383);
-return x_388;
-}
-else
-{
-lean_object* x_389; uint8_t x_390; 
-x_389 = lean_ctor_get(x_386, 0);
-lean_inc(x_389);
-lean_dec(x_386);
-x_390 = l_Lean_Expr_hasLooseBVars(x_389);
-if (x_390 == 0)
-{
-lean_object* x_391; lean_object* x_392; 
-x_391 = lean_box(0);
-lean_inc(x_389);
-x_392 = l_Lean_FindMVar_main___at___private_Lean_Elab_App_0__Lean_Elab_Term_ElabAppArgs_propagateExpectedType___spec__1(x_343, x_389, x_391);
-if (lean_obj_tag(x_392) == 0)
-{
-lean_object* x_393; lean_object* x_394; 
-lean_dec(x_389);
-lean_dec(x_378);
-lean_dec(x_351);
-lean_dec(x_7);
-lean_dec(x_6);
-lean_dec(x_5);
-lean_dec(x_4);
-lean_dec(x_3);
-lean_dec(x_2);
-lean_dec(x_1);
-x_393 = lean_box(0);
-if (lean_is_scalar(x_377)) {
- x_394 = lean_alloc_ctor(0, 2, 0);
-} else {
- x_394 = x_377;
-}
-lean_ctor_set(x_394, 0, x_393);
-lean_ctor_set(x_394, 1, x_383);
-return x_394;
-}
-else
-{
-lean_object* x_395; 
-lean_dec(x_392);
-lean_inc(x_389);
-x_395 = l_Lean_FindMVar_main___at___private_Lean_Elab_App_0__Lean_Elab_Term_ElabAppArgs_propagateExpectedType___spec__2(x_351, x_389, x_391);
-if (lean_obj_tag(x_395) == 0)
-{
-lean_object* x_396; lean_object* x_397; 
-lean_dec(x_377);
-x_396 = l___private_Lean_Elab_App_0__Lean_Elab_Term_ElabAppArgs_hasOptAutoParams___closed__1;
-lean_inc(x_7);
-lean_inc(x_6);
-lean_inc(x_5);
-lean_inc(x_4);
-lean_inc(x_3);
-lean_inc(x_2);
-lean_inc(x_1);
-lean_inc(x_389);
-x_397 = l_Lean_Meta_forallTelescopeReducing___at___private_Lean_Elab_App_0__Lean_Elab_Term_ElabAppArgs_hasOptAutoParams___spec__2___rarg(x_389, x_396, x_1, x_2, x_3, x_4, x_5, x_6, x_7, x_383);
-if (lean_obj_tag(x_397) == 0)
-{
-lean_object* x_398; lean_object* x_399; lean_object* x_400; uint8_t x_401; lean_object* x_402; uint8_t x_433; 
-x_398 = lean_ctor_get(x_397, 0);
-lean_inc(x_398);
-x_399 = lean_ctor_get(x_397, 1);
-lean_inc(x_399);
-if (lean_is_exclusive(x_397)) {
- lean_ctor_release(x_397, 0);
- lean_ctor_release(x_397, 1);
- x_400 = x_397;
-} else {
- lean_dec_ref(x_397);
- x_400 = lean_box(0);
-}
-x_433 = lean_unbox(x_398);
-lean_dec(x_398);
-if (x_433 == 0)
-{
-lean_object* x_434; lean_object* x_435; lean_object* x_436; uint8_t x_437; 
-lean_dec(x_400);
-x_434 = lean_st_ref_get(x_7, x_399);
-x_435 = lean_ctor_get(x_434, 0);
-lean_inc(x_435);
-x_436 = lean_ctor_get(x_435, 3);
-lean_inc(x_436);
-lean_dec(x_435);
-x_437 = lean_ctor_get_uint8(x_436, sizeof(void*)*1);
-lean_dec(x_436);
-if (x_437 == 0)
-{
-lean_object* x_438; uint8_t x_439; 
-x_438 = lean_ctor_get(x_434, 1);
-lean_inc(x_438);
-lean_dec(x_434);
-x_439 = 0;
-x_401 = x_439;
-x_402 = x_438;
-goto block_432;
-}
-else
-{
-lean_object* x_440; lean_object* x_441; lean_object* x_442; lean_object* x_443; lean_object* x_444; uint8_t x_445; 
-x_440 = lean_ctor_get(x_434, 1);
-lean_inc(x_440);
-lean_dec(x_434);
-x_441 = l___private_Lean_Elab_App_0__Lean_Elab_Term_ElabAppArgs_propagateExpectedType___closed__3;
-x_442 = l___private_Lean_Util_Trace_0__Lean_checkTraceOptionM___at___private_Lean_Elab_App_0__Lean_Elab_Term_ElabAppArgs_propagateExpectedType___spec__7(x_441, x_1, x_2, x_3, x_4, x_5, x_6, x_7, x_440);
-x_443 = lean_ctor_get(x_442, 0);
-lean_inc(x_443);
-x_444 = lean_ctor_get(x_442, 1);
-lean_inc(x_444);
-lean_dec(x_442);
-x_445 = lean_unbox(x_443);
-lean_dec(x_443);
-x_401 = x_445;
-x_402 = x_444;
-goto block_432;
-}
-}
-else
-{
-lean_object* x_446; lean_object* x_447; 
-lean_dec(x_389);
-lean_dec(x_378);
-lean_dec(x_7);
-lean_dec(x_6);
-lean_dec(x_5);
-lean_dec(x_4);
-lean_dec(x_3);
-lean_dec(x_2);
-lean_dec(x_1);
-x_446 = lean_box(0);
-if (lean_is_scalar(x_400)) {
- x_447 = lean_alloc_ctor(0, 2, 0);
-} else {
- x_447 = x_400;
-}
-lean_ctor_set(x_447, 0, x_446);
-lean_ctor_set(x_447, 1, x_399);
-return x_447;
-}
-block_432:
-{
-if (x_401 == 0)
-{
-lean_object* x_403; 
-x_403 = l_Lean_Meta_isExprDefEq___at___private_Lean_Elab_App_0__Lean_Elab_Term_ElabAppArgs_propagateExpectedType___spec__3(x_378, x_389, x_1, x_2, x_3, x_4, x_5, x_6, x_7, x_402);
-lean_dec(x_3);
-lean_dec(x_2);
-lean_dec(x_1);
-if (lean_obj_tag(x_403) == 0)
-{
-lean_object* x_404; lean_object* x_405; lean_object* x_406; lean_object* x_407; 
-x_404 = lean_ctor_get(x_403, 1);
-lean_inc(x_404);
-if (lean_is_exclusive(x_403)) {
- lean_ctor_release(x_403, 0);
- lean_ctor_release(x_403, 1);
- x_405 = x_403;
-} else {
- lean_dec_ref(x_403);
- x_405 = lean_box(0);
-}
-x_406 = lean_box(0);
-if (lean_is_scalar(x_405)) {
- x_407 = lean_alloc_ctor(0, 2, 0);
-} else {
- x_407 = x_405;
-}
-lean_ctor_set(x_407, 0, x_406);
-lean_ctor_set(x_407, 1, x_404);
-return x_407;
-}
-else
-{
-lean_object* x_408; lean_object* x_409; lean_object* x_410; lean_object* x_411; 
-x_408 = lean_ctor_get(x_403, 0);
-lean_inc(x_408);
-x_409 = lean_ctor_get(x_403, 1);
-lean_inc(x_409);
-if (lean_is_exclusive(x_403)) {
- lean_ctor_release(x_403, 0);
- lean_ctor_release(x_403, 1);
- x_410 = x_403;
-} else {
- lean_dec_ref(x_403);
- x_410 = lean_box(0);
-}
-if (lean_is_scalar(x_410)) {
- x_411 = lean_alloc_ctor(1, 2, 0);
-} else {
- x_411 = x_410;
-}
-lean_ctor_set(x_411, 0, x_408);
-lean_ctor_set(x_411, 1, x_409);
-return x_411;
-}
-}
-else
-{
-lean_object* x_412; lean_object* x_413; lean_object* x_414; lean_object* x_415; lean_object* x_416; lean_object* x_417; lean_object* x_418; lean_object* x_419; lean_object* x_420; lean_object* x_421; lean_object* x_422; lean_object* x_423; 
-lean_inc(x_378);
-x_412 = lean_alloc_ctor(2, 1, 0);
-lean_ctor_set(x_412, 0, x_378);
-x_413 = l_Array_foldlMUnsafe_fold___at_Lean_withNestedTraces___spec__5___closed__1;
-x_414 = lean_alloc_ctor(10, 2, 0);
-lean_ctor_set(x_414, 0, x_413);
-lean_ctor_set(x_414, 1, x_412);
-x_415 = l_Lean_Meta_isLevelDefEqAux___closed__6;
-x_416 = lean_alloc_ctor(10, 2, 0);
-lean_ctor_set(x_416, 0, x_414);
-lean_ctor_set(x_416, 1, x_415);
-lean_inc(x_389);
-x_417 = lean_alloc_ctor(2, 1, 0);
-lean_ctor_set(x_417, 0, x_389);
-x_418 = lean_alloc_ctor(10, 2, 0);
-lean_ctor_set(x_418, 0, x_416);
-lean_ctor_set(x_418, 1, x_417);
-x_419 = lean_alloc_ctor(10, 2, 0);
-lean_ctor_set(x_419, 0, x_418);
-lean_ctor_set(x_419, 1, x_413);
-x_420 = l___private_Lean_Elab_App_0__Lean_Elab_Term_ElabAppArgs_propagateExpectedType___closed__3;
-x_421 = l_Lean_addTrace___at___private_Lean_Elab_App_0__Lean_Elab_Term_ElabAppArgs_propagateExpectedType___spec__6(x_420, x_419, x_1, x_2, x_3, x_4, x_5, x_6, x_7, x_402);
-x_422 = lean_ctor_get(x_421, 1);
-lean_inc(x_422);
-lean_dec(x_421);
-x_423 = l_Lean_Meta_isExprDefEq___at___private_Lean_Elab_App_0__Lean_Elab_Term_ElabAppArgs_propagateExpectedType___spec__3(x_378, x_389, x_1, x_2, x_3, x_4, x_5, x_6, x_7, x_422);
-lean_dec(x_3);
-lean_dec(x_2);
-lean_dec(x_1);
-if (lean_obj_tag(x_423) == 0)
-{
-lean_object* x_424; lean_object* x_425; lean_object* x_426; lean_object* x_427; 
-x_424 = lean_ctor_get(x_423, 1);
-lean_inc(x_424);
-if (lean_is_exclusive(x_423)) {
- lean_ctor_release(x_423, 0);
- lean_ctor_release(x_423, 1);
- x_425 = x_423;
-} else {
- lean_dec_ref(x_423);
- x_425 = lean_box(0);
-}
-x_426 = lean_box(0);
-if (lean_is_scalar(x_425)) {
- x_427 = lean_alloc_ctor(0, 2, 0);
-} else {
- x_427 = x_425;
-}
-lean_ctor_set(x_427, 0, x_426);
-lean_ctor_set(x_427, 1, x_424);
-return x_427;
-}
-else
-{
-lean_object* x_428; lean_object* x_429; lean_object* x_430; lean_object* x_431; 
-x_428 = lean_ctor_get(x_423, 0);
-lean_inc(x_428);
-x_429 = lean_ctor_get(x_423, 1);
-lean_inc(x_429);
-if (lean_is_exclusive(x_423)) {
- lean_ctor_release(x_423, 0);
- lean_ctor_release(x_423, 1);
- x_430 = x_423;
-} else {
- lean_dec_ref(x_423);
- x_430 = lean_box(0);
-}
-if (lean_is_scalar(x_430)) {
- x_431 = lean_alloc_ctor(1, 2, 0);
-} else {
- x_431 = x_430;
-}
-lean_ctor_set(x_431, 0, x_428);
-lean_ctor_set(x_431, 1, x_429);
-return x_431;
-}
-}
-}
-}
-else
-{
-lean_object* x_448; lean_object* x_449; lean_object* x_450; lean_object* x_451; 
-lean_dec(x_389);
-lean_dec(x_378);
-lean_dec(x_7);
-lean_dec(x_6);
-lean_dec(x_5);
-lean_dec(x_4);
-lean_dec(x_3);
-lean_dec(x_2);
-lean_dec(x_1);
-x_448 = lean_ctor_get(x_397, 0);
-lean_inc(x_448);
-x_449 = lean_ctor_get(x_397, 1);
-lean_inc(x_449);
-if (lean_is_exclusive(x_397)) {
- lean_ctor_release(x_397, 0);
- lean_ctor_release(x_397, 1);
- x_450 = x_397;
-} else {
- lean_dec_ref(x_397);
- x_450 = lean_box(0);
-}
-if (lean_is_scalar(x_450)) {
- x_451 = lean_alloc_ctor(1, 2, 0);
-} else {
- x_451 = x_450;
-}
-lean_ctor_set(x_451, 0, x_448);
-lean_ctor_set(x_451, 1, x_449);
-return x_451;
-}
-}
-else
-{
-lean_object* x_452; lean_object* x_453; 
-lean_dec(x_395);
-lean_dec(x_389);
-lean_dec(x_378);
-lean_dec(x_7);
-lean_dec(x_6);
-lean_dec(x_5);
-lean_dec(x_4);
-lean_dec(x_3);
-lean_dec(x_2);
-lean_dec(x_1);
-x_452 = lean_box(0);
-if (lean_is_scalar(x_377)) {
- x_453 = lean_alloc_ctor(0, 2, 0);
-} else {
- x_453 = x_377;
-}
-lean_ctor_set(x_453, 0, x_452);
-lean_ctor_set(x_453, 1, x_383);
-return x_453;
-}
-}
-}
-else
-{
-lean_object* x_454; lean_object* x_455; 
-lean_dec(x_389);
-lean_dec(x_378);
-lean_dec(x_351);
-lean_dec(x_343);
-lean_dec(x_7);
-lean_dec(x_6);
-lean_dec(x_5);
-lean_dec(x_4);
-lean_dec(x_3);
-lean_dec(x_2);
-lean_dec(x_1);
-x_454 = lean_box(0);
-if (lean_is_scalar(x_377)) {
- x_455 = lean_alloc_ctor(0, 2, 0);
-} else {
- x_455 = x_377;
-}
-lean_ctor_set(x_455, 0, x_454);
-lean_ctor_set(x_455, 1, x_383);
-return x_455;
-}
-}
-}
-block_479:
-{
-if (x_457 == 0)
-{
-lean_dec(x_346);
-x_383 = x_458;
-goto block_456;
-}
-else
-{
-lean_object* x_459; lean_object* x_460; lean_object* x_461; lean_object* x_462; lean_object* x_463; lean_object* x_464; lean_object* x_465; lean_object* x_466; lean_object* x_467; lean_object* x_468; lean_object* x_469; lean_object* x_470; lean_object* x_471; lean_object* x_472; lean_object* x_473; lean_object* x_474; lean_object* x_475; lean_object* x_476; lean_object* x_477; lean_object* x_478; 
-x_459 = lean_array_get_size(x_346);
-lean_dec(x_346);
-x_460 = l_Lean_fmt___at_Lean_Position_instToFormatPosition___spec__1(x_459);
-x_461 = lean_alloc_ctor(0, 1, 0);
-lean_ctor_set(x_461, 0, x_460);
-x_462 = l___private_Lean_Elab_App_0__Lean_Elab_Term_ElabAppArgs_propagateExpectedType___closed__5;
-x_463 = lean_alloc_ctor(10, 2, 0);
-lean_ctor_set(x_463, 0, x_462);
-lean_ctor_set(x_463, 1, x_461);
-x_464 = l___private_Lean_Elab_App_0__Lean_Elab_Term_ElabAppArgs_propagateExpectedType___closed__7;
-x_465 = lean_alloc_ctor(10, 2, 0);
-lean_ctor_set(x_465, 0, x_463);
-lean_ctor_set(x_465, 1, x_464);
-lean_inc(x_382);
-x_466 = l_Lean_fmt___at_Lean_Position_instToFormatPosition___spec__1(x_382);
-x_467 = lean_alloc_ctor(0, 1, 0);
-lean_ctor_set(x_467, 0, x_466);
-x_468 = lean_alloc_ctor(10, 2, 0);
-lean_ctor_set(x_468, 0, x_465);
-lean_ctor_set(x_468, 1, x_467);
-x_469 = l___private_Lean_Elab_App_0__Lean_Elab_Term_ElabAppArgs_propagateExpectedType___closed__9;
-x_470 = lean_alloc_ctor(10, 2, 0);
-lean_ctor_set(x_470, 0, x_468);
-lean_ctor_set(x_470, 1, x_469);
-x_471 = lean_ctor_get(x_343, 1);
-lean_inc(x_471);
-x_472 = lean_alloc_ctor(2, 1, 0);
-lean_ctor_set(x_472, 0, x_471);
-x_473 = lean_alloc_ctor(10, 2, 0);
-lean_ctor_set(x_473, 0, x_470);
-lean_ctor_set(x_473, 1, x_472);
-x_474 = l_Array_foldlMUnsafe_fold___at_Lean_withNestedTraces___spec__5___closed__1;
-x_475 = lean_alloc_ctor(10, 2, 0);
-lean_ctor_set(x_475, 0, x_473);
-lean_ctor_set(x_475, 1, x_474);
-x_476 = l___private_Lean_Elab_App_0__Lean_Elab_Term_ElabAppArgs_propagateExpectedType___closed__3;
-x_477 = l_Lean_addTrace___at___private_Lean_Elab_App_0__Lean_Elab_Term_ElabAppArgs_propagateExpectedType___spec__6(x_476, x_475, x_1, x_2, x_3, x_4, x_5, x_6, x_7, x_458);
-x_478 = lean_ctor_get(x_477, 1);
-lean_inc(x_478);
-lean_dec(x_477);
-x_383 = x_478;
-goto block_456;
-}
-}
-}
-else
-{
-lean_object* x_492; lean_object* x_493; 
-lean_dec(x_378);
-lean_dec(x_351);
-lean_dec(x_346);
-lean_dec(x_343);
-lean_dec(x_7);
-lean_dec(x_6);
-lean_dec(x_5);
-lean_dec(x_4);
-lean_dec(x_3);
-lean_dec(x_2);
-lean_dec(x_1);
-x_492 = lean_box(0);
-if (lean_is_scalar(x_377)) {
- x_493 = lean_alloc_ctor(0, 2, 0);
-} else {
- x_493 = x_377;
-}
-lean_ctor_set(x_493, 0, x_492);
-lean_ctor_set(x_493, 1, x_376);
-return x_493;
-}
-}
-}
-else
-{
-lean_object* x_494; lean_object* x_495; 
-lean_dec(x_351);
-lean_dec(x_346);
-lean_dec(x_343);
-lean_dec(x_7);
-lean_dec(x_6);
-lean_dec(x_5);
-lean_dec(x_4);
-lean_dec(x_3);
-lean_dec(x_2);
-lean_dec(x_1);
-x_494 = lean_box(0);
-x_495 = lean_alloc_ctor(0, 2, 0);
-lean_ctor_set(x_495, 0, x_494);
-lean_ctor_set(x_495, 1, x_344);
-return x_495;
-}
-}
-else
-{
-lean_object* x_496; lean_object* x_497; 
-lean_dec(x_346);
-lean_dec(x_343);
-lean_dec(x_7);
-lean_dec(x_6);
-lean_dec(x_5);
-lean_dec(x_4);
-lean_dec(x_3);
-lean_dec(x_2);
-lean_dec(x_1);
-x_496 = lean_box(0);
-x_497 = lean_alloc_ctor(0, 2, 0);
-lean_ctor_set(x_497, 0, x_496);
-lean_ctor_set(x_497, 1, x_344);
-return x_497;
-}
-}
-else
-{
-lean_object* x_498; lean_object* x_499; 
-lean_dec(x_346);
-lean_dec(x_343);
-lean_dec(x_7);
-lean_dec(x_6);
-lean_dec(x_5);
-lean_dec(x_4);
-lean_dec(x_3);
-lean_dec(x_2);
-lean_dec(x_1);
-x_498 = lean_box(0);
-x_499 = lean_alloc_ctor(0, 2, 0);
-lean_ctor_set(x_499, 0, x_498);
-lean_ctor_set(x_499, 1, x_344);
-return x_499;
-}
+ x_267 = x_12;
+}
+lean_ctor_set(x_267, 0, x_266);
+lean_ctor_set(x_267, 1, x_11);
+return x_267;
 }
 }
 }
@@ -36261,7 +35111,7 @@ _start:
 lean_object* x_1; lean_object* x_2; lean_object* x_3; lean_object* x_4; lean_object* x_5; lean_object* x_6; 
 x_1 = l_Array_mapMUnsafe_map___at___private_Lean_Elab_App_0__Lean_Elab_Term_mergeFailures___spec__1___closed__1;
 x_2 = l_Array_mapMUnsafe_map___at___private_Lean_Elab_App_0__Lean_Elab_Term_mergeFailures___spec__1___closed__2;
-x_3 = lean_unsigned_to_nat(825u);
+x_3 = lean_unsigned_to_nat(827u);
 x_4 = lean_unsigned_to_nat(35u);
 x_5 = l_Lean_Syntax_strLitToAtom___closed__3;
 x_6 = l___private_Init_Util_0__mkPanicMessageWithDecl(x_1, x_2, x_3, x_4, x_5);
@@ -36549,7 +35399,7 @@ _start:
 lean_object* x_1; lean_object* x_2; lean_object* x_3; lean_object* x_4; lean_object* x_5; lean_object* x_6; 
 x_1 = l_Array_mapMUnsafe_map___at___private_Lean_Elab_App_0__Lean_Elab_Term_mergeFailures___spec__1___closed__1;
 x_2 = l_Array_mapMUnsafe_map___at___private_Lean_Elab_App_0__Lean_Elab_Term_elabAppAux___spec__1___closed__1;
-x_3 = lean_unsigned_to_nat(843u);
+x_3 = lean_unsigned_to_nat(845u);
 x_4 = lean_unsigned_to_nat(35u);
 x_5 = l_Lean_Syntax_strLitToAtom___closed__3;
 x_6 = l___private_Init_Util_0__mkPanicMessageWithDecl(x_1, x_2, x_3, x_4, x_5);
@@ -38461,7 +37311,7 @@ x_5 = l_Lean_KeyedDeclsAttribute_addBuiltin___rarg(x_2, x_3, x_4, x_1);
 return x_5;
 }
 }
-lean_object* l_Lean_Elab_Term_initFn____x40_Lean_Elab_App___hyg_7555_(lean_object* x_1) {
+lean_object* l_Lean_Elab_Term_initFn____x40_Lean_Elab_App___hyg_7569_(lean_object* x_1) {
 _start:
 {
 lean_object* x_2; lean_object* x_3; 
@@ -38800,7 +37650,7 @@ lean_mark_persistent(l___regBuiltin_Lean_Elab_Term_elabArrayRef___closed__1);
 res = l___regBuiltin_Lean_Elab_Term_elabArrayRef(lean_io_mk_world());
 if (lean_io_result_is_error(res)) return res;
 lean_dec_ref(res);
-res = l_Lean_Elab_Term_initFn____x40_Lean_Elab_App___hyg_7555_(lean_io_mk_world());
+res = l_Lean_Elab_Term_initFn____x40_Lean_Elab_App___hyg_7569_(lean_io_mk_world());
 if (lean_io_result_is_error(res)) return res;
 lean_dec_ref(res);
 return lean_io_result_mk_ok(lean_box(0));
